src/Soundness.v
@@ -1,4 +1,4 @@
-From TLC Require Import LibString LibList LibLN.
+From TLC Require Import LibString LibOption LibList LibLN.
 From MCore Require Import
      Syntax SyntaxProps Typing TypingProps
      SmallStep SmallStepProps Tactics.
@@ -20,27 +20,39 @@ Module Soundness (P : PAT).
           Gamma |= t ~: ty ->
           t --> t' ->
           Gamma |= t' ~: ty.
-      Proof.
+      Proof with eauto using ok_type_lct with mcore.
         introv hasType Hstep.
         gen t'.
-        induction hasType; intros; inverts~ Hstep ;
-          try (with_hyp (is_context _) as ctx ; with_hyp (_ = _) as eq
-               ; inverts ctx ; inverts* eq).
+        induction hasType; intros; inverts Hstep ;
+          try (with_hyp (is_context _) as ctx ; with_hyp (_ = _) as eq ;
+               inverts ctx ; inverts eq)...
         { Case "TmApp". inverts hasType1.
           pick_fresh x. rewrite~ (subst_intro x).
-          apply_empty~ ok_term_subst. }
+          apply_empty* ok_term_subst. }
         { Case "TmTyApp". inverts hasType.
           pick_fresh X.
-          rewrite* (tsubst_intro X).
-          rewrite* (tsubst_t_intro X).
-          apply_empty~ ok_term_tsubst. }
+          rewrite (tsubst_intro X)...
+          rewrite (tsubst_t_intro X)...
+          apply_empty* ok_term_tsubst. }
         { Case "TmFix". inverts hasType.
           pick_fresh x. rewrite~ (subst_intro x).
           apply_empty* ok_term_subst. }
         { Case "TmProj1". inverts* hasType. }
         { Case "TmProj2". inverts* hasType. }
-        { Case "TmMatchThen". pick_fresh x. rewrite~ (subst_intro x).
-          apply_empty~ ok_term_subst. apply* match1_ok_pat. }
+        { Case "TmMatchThen". pick_fresh M. pick_fresh x. rewrite~ (subst_intro x).
+          assert (Gamma & M ~ BindMatch t p true |= [x => v'] ([0 ~> TmFVar x] t1) ~: ty2).
+          { apply_empty~ ok_term_subst ; try constructors*. apply* match1_ok_pat.
+            apply_empty~ ok_pat_weakening ; try constructors*. apply H. }
+          replaces true with (is_some (match1 t p)) in H4. rewrite~ H10.
+          apply_empty ok_term_drop_match... }
+        { Case "TmMatchElse". pick_fresh M.
+          replaces false with (is_some (match1 t p)) in H2. rewrite~ H10.
+          apply_empty ok_term_drop_match... applys~ H2 M. }
+        { Case "TmMatchCong". forwards* Htk : ok_pat_ok_type.
+          apply_fresh TMatch ; intros...
+          - applys~ ok_term_step_match t.
+            constructor~. constructors... apply_empty~ ok_type_weakening. constructors...
+          - apply_empty~ ok_term_step_match. constructors... }
         { Case "TmType". pick_fresh T. applys* ok_term_Topen_push T t. }
         { Case "TmTypeCong". apply_fresh TType as T' ; auto. }
         { Case "TmConDef". pick_fresh K. applys* ok_term_Kopen_push K t. }
@@ -49,7 +61,7 @@ Module Soundness (P : PAT).
           assert (i < length ps0) by apply* matchN_length.
           forwards* (L&ty1'&Hpat&Htype) : ok_term_get_cases_inv i.
           remember (nth i bs) ; pick_fresh x ; substs. rewrite~ (subst_intro x).
-          apply_empty~ ok_term_subst. apply* matchN_ok_pat. }
+          apply_empty* ok_term_subst. apply* matchN_ok_pat. }
       Qed.
 
       Definition no_vars (Gamma : env) : Prop :=
@@ -58,10 +70,11 @@ Module Soundness (P : PAT).
       Theorem progress :
         forall Gamma t ty,
           no_vars Gamma ->
+          ~ contradictory Gamma ->
           Gamma |= t ~: ty ->
           is_value t \/ exists t', t --> t'.
       Proof.
-        introv Hnv hasType.
+        introv Hnv Hnc hasType.
         induction hasType; substs*.
         { Case "TmFVar". false. apply* Hnv. }
         { Case "TmApp". right.
@@ -86,11 +99,12 @@ Module Soundness (P : PAT).
         { Case "TmCon".
           forwards* [Hval | (t' & Hstep)]: IHhasType. }
         { Case "TmMatch". right.
-          forwards* [Hval | (t' & Hstep)]: IHhasType1.
+          forwards* [Hval | (t' & Hstep)]: IHhasType.
           destruct (match1 t p) eqn:Hmatch ; auto_star. }
         { Case "TmType". right. pick_fresh T.
           forwards* [Hval | (t' & Hstep)]: H0 T.
           + introv Hb. binds_cases Hb. apply* Hnv.
+          + intro. apply Hnc. apply_empty* (contradictory_tname_strengthening T).
           + forwards* Hval' : Topen_is_value Hval.
           + rewrite <- (Topen_t_Tclose 0 T t') in Hstep.
             * eexists. apply_fresh ETypeCong.
@@ -99,6 +113,7 @@ Module Soundness (P : PAT).
         { Case "TmConDef". right. pick_fresh K.
           forwards* [Hval | (t' & Hstep)]: H3 K.
           + introv Hb. binds_cases Hb. apply* Hnv.
+          + intro. apply Hnc. apply_empty* (contradictory_con_strengthening K).
           + forwards* Hval' : Kopen_is_value Hval.
           + rewrite <- (Kopen_t_Kclose 0 K t') in Hstep.
             * eexists. apply_fresh EConDefCong.
