src/Tactics.v
@@ -1,4 +1,4 @@
-From TLC Require Import LibVar.
+From TLC Require Import LibEnv LibVar.
 From TLC Require Export LibTactics.
 
 Create HintDb mcore.
@@ -9,6 +9,13 @@ Ltac auto_star ::= try solve [ auto with mcore
 Ltac solve_var := repeat (simpls ; try cases_if ; auto_star ; try notin_false).
 
 Ltac solve_eq t := induction t ; intros ; solve_var ; fequals*.
+
+(* Tactic used to extract information from hypotheses on the form *)
+(* Gamma & X ~ b1 = G1 & Y ~ b2 & G2 *)
+Ltac fiddle_env G2 Heq :=
+  destruct G2 using env_ind ; rew_env_concat in Heq ;
+  forwards (?&?&?): eq_push_inv Heq ; fequals ; substs ;
+  autorewrite with rew_env_map rew_env_concat.
 
 (* Rename a hypothesis in scope based on a pattern matching its type. *)
 Tactic Notation "with_hyp" open_constr(P) "as" ident(X) :=
