src/TypingProps.v
@@ -32,33 +32,71 @@ Module TypingProps (P : PAT).
           ok_env (G1 & G2 & G3) ->
           ok_pat (G1 & G2 & G3) p T T'.
 
-      Parameter pats_exhaustive_weakening :
+      Parameter exhaustive_weakening :
         forall G3 G1 G2 ps T,
-          pats_exhaustive (G1 & G3) ps T ->
+          exhaustive (G1 & G3) ps T ->
           ok_env (G1 & G2 & G3) ->
-          pats_exhaustive (G1 & G2 & G3) ps T.
+          exhaustive (G1 & G2 & G3) ps T.
+
+      Parameter contradictory_weakening :
+        forall G3 G1 G2,
+          contradictory (G1 & G3) ->
+          ok_env (G1 & G2 & G3) ->
+          contradictory (G1 & G2 & G3).
 
       Parameter ok_pat_strengthening :
         forall G1 G2 x p T1 T1' T2,
           ok_pat (G1 & x ~ BindVar T2 & G2) p T1 T1' ->
           ok_pat (G1 & G2) p T1 T1'.
 
-      Parameter pats_exhaustive_strengthening :
+      Parameter ok_pat_bsubst :
+        forall G1 G2 p x t T T',
+          ok_pat (G1 & G2) p T T' ->
+          ok_pat (G1 & map (bsubst x t) G2) p T T'.
+
+      Parameter exhaustive_strengthening :
         forall G1 G2 x ps T1 T2,
-          pats_exhaustive (G1 & x ~ BindVar T2 & G2) ps T1 ->
-          pats_exhaustive (G1 & G2) ps T1.
+          exhaustive (G1 & x ~ BindVar T2 & G2) ps T1 ->
+          exhaustive (G1 & G2) ps T1.
+
+      Parameter exhaustive_bsubst :
+        forall G1 G2 x t ps T1,
+          exhaustive (G1 & G2) ps T1 ->
+          exhaustive (G1 & map (bsubst x t) G2) ps T1.
+
+      Parameter contradictory_subst :
+        forall G1 G2 x u T,
+          contradictory (G1 & x ~ BindVar T & G2) ->
+          G1 |= u ~: T ->
+          contradictory (G1 & map (bsubst x u) G2).
+
+      Parameter ok_pat_match_strengthening :
+        forall M G2 G1 t p' m ty ty' p,
+          ok_pat (G1 & M ~ BindMatch t p' m & G2) p ty ty' ->
+          ok_pat (G1 & G2) p ty ty'.
+
+      Parameter exhaustive_match_strengthening :
+        forall M G2 G1 t p' m ty ps,
+          exhaustive (G1 & M ~ BindMatch t p' m & G2) ps ty ->
+          exhaustive (G1 & G2) ps ty.
 
       Parameter ok_pat_tsubst :
         forall G1 G2 p X U T T' k,
           ok_pat (G1 & X ~ BindTVar k & G2) p T T' ->
           G1 |= U ~:: k ->
-          ok_pat (G1 & map (bsubst X U) G2) p ({X => U}T) ({X => U}T').
+          ok_pat (G1 & map (tbsubst X U) G2) p ({X => U}T) ({X => U}T').
 
-      Parameter pats_exhaustive_tsubst :
+      Parameter exhaustive_tsubst :
         forall G1 G2 ps X U ty k,
-          pats_exhaustive (G1 & X ~ BindTVar k & G2) ps ty ->
+          exhaustive (G1 & X ~ BindTVar k & G2) ps ty ->
           G1 |= U ~:: k ->
-          pats_exhaustive (G1 & map (bsubst X U) G2) ps ({X => U} ty).
+          exhaustive (G1 & map (tbsubst X U) G2) ps ({X => U} ty).
+
+      Parameter contradictory_tsubst :
+        forall G1 G2 X U k,
+          contradictory (G1 & X ~ BindTVar k & G2) ->
+          G1 |= U ~:: k ->
+          contradictory (G1 & map (tbsubst X U) G2).
 
       Parameter ok_pat_comm :
         forall G1 G2 x1 x2 b1 b2 p T T',
@@ -66,11 +104,17 @@ Module TypingProps (P : PAT).
           ok_env (G1 & x2 ~ b2 & x1 ~ b1 & G2) ->
           ok_pat (G1 & x2 ~ b2 & x1 ~ b1 & G2) p T T'.
 
-      Parameter pats_exhaustive_comm :
+      Parameter exhaustive_comm :
         forall G1 G2 x1 x2 b1 b2 ps T,
-          pats_exhaustive (G1 & x1 ~ b1 & x2 ~ b2 & G2) ps T ->
+          exhaustive (G1 & x1 ~ b1 & x2 ~ b2 & G2) ps T ->
           ok_env (G1 & x2 ~ b2 & x1 ~ b1 & G2) ->
-          pats_exhaustive (G1 & x2 ~ b2 & x1 ~ b1 & G2) ps T.
+          exhaustive (G1 & x2 ~ b2 & x1 ~ b1 & G2) ps T.
+
+      Parameter contradictory_comm :
+        forall G1 G2 x1 x2 b1 b2,
+          contradictory (G1 & x1 ~ b1 & x2 ~ b2 & G2) ->
+          ok_env (G1 & x2 ~ b2 & x1 ~ b1 & G2) ->
+          contradictory (G1 & x2 ~ b2 & x1 ~ b1 & G2).
 
       Parameter ok_pat_tname_strengthening :
         forall T G2 G1 ty ty' p,
@@ -78,6 +122,12 @@ Module TypingProps (P : PAT).
           ok_pat (G1 & T ~ BindTName & G2) p ty ty' ->
           ok_env (G1 & G2) ->
           ok_pat (G1 & G2) p ty ty'.
+
+      Parameter contradictory_tname_strengthening :
+        forall T G2 G1,
+          contradictory (G1 & T ~ BindTName & G2) ->
+          ok_env (G1 & G2) ->
+          contradictory (G1 & G2).
 
       Parameter ok_pat_Tsubst :
         forall G2 G1 T T' p ty ty',
@@ -87,13 +137,20 @@ Module TypingProps (P : PAT).
           ok_pat (G1 & T' ~ BindTName & map (Tbsubst T (FTName T')) G2)
                  p (Tsubst_ty T (FTName T') ty) (Tsubst_ty T (FTName T') ty').
 
-      Parameter pats_exhaustive_Tsubst :
+      Parameter exhaustive_Tsubst :
         forall G1 G2 ps T T' ty,
-          pats_exhaustive (G1 & T ~ BindTName & G2) ps ty ->
+          exhaustive (G1 & T ~ BindTName & G2) ps ty ->
           T' # G1 & T ~ BindTName & G2 ->
           ok_env (G1 & T ~ BindTName & G2) ->
-          pats_exhaustive (G1 & T' ~ BindTName & map (Tbsubst T (FTName T')) G2)
+          exhaustive (G1 & T' ~ BindTName & map (Tbsubst T (FTName T')) G2)
                           ps (Tsubst_ty T (FTName T') ty).
+
+      Parameter contradictory_Tsubst :
+        forall G1 G2 T T',
+          contradictory (G1 & T ~ BindTName & G2) ->
+          T' # G1 & T ~ BindTName & G2 ->
+          ok_env (G1 & T ~ BindTName & G2) ->
+          contradictory (G1 & T' ~ BindTName & map (Tbsubst T (FTName T')) G2).
 
       Parameter ok_pat_con_strengthening :
         forall K G2 G1 d0 ty0 T ty ty' p,
@@ -101,6 +158,12 @@ Module TypingProps (P : PAT).
           ok_pat (G1 & K ~ BindCon d0 ty0 T & G2) p ty ty' ->
           ok_env (G1 & G2) ->
           ok_pat (G1 & G2) p ty ty'.
+
+      Parameter contradictory_con_strengthening :
+        forall K G2 G1 d0 ty0 T,
+          contradictory (G1 & K ~ BindCon d0 ty0 T & G2) ->
+          ok_env (G1 & G2) ->
+          contradictory (G1 & G2).
 
       Parameter ok_pat_notin_K :
         forall Gamma p ty ty' X,
@@ -116,19 +179,26 @@ Module TypingProps (P : PAT).
           ok_pat (G1 & K' ~ BindCon d0 ty0 T & map (Kbsubst K (FCon K')) G2)
                  (Ksubst_p K (FCon K') p) (Ksubst_ty K (FCon K') ty) (Ksubst_ty K (FCon K') ty').
 
-      Parameter pats_compatible_Ksubst :
+      Parameter compatible_Ksubst :
         forall ps K K',
           K' \notin fold varsM Kfv_p ps ->
-          pats_compatible ps ->
-          pats_compatible (LibList.map (Ksubst_p K (FCon K')) ps).
+          compatible ps ->
+          compatible (LibList.map (Ksubst_p K (FCon K')) ps).
 
-      Parameter pats_exhaustive_Ksubst :
+      Parameter exhaustive_Ksubst :
         forall G1 G2 ps K K' d ty' T ty,
-          pats_exhaustive (G1 & K ~ BindCon d ty' T & G2) ps ty ->
+          exhaustive (G1 & K ~ BindCon d ty' T & G2) ps ty ->
           K' # G1 & K ~ BindCon d ty' T & G2 ->
           ok_env (G1 & K ~ BindCon d ty' T & G2) ->
-          pats_exhaustive (G1 & K' ~ BindCon d ty' T & map (Kbsubst K (FCon K')) G2)
+          exhaustive (G1 & K' ~ BindCon d ty' T & map (Kbsubst K (FCon K')) G2)
                           (LibList.map (Ksubst_p K (FCon K')) ps) (Ksubst_ty K (FCon K') ty).
+
+      Parameter contradictory_Ksubst :
+        forall G1 G2 K K' d ty' T,
+          contradictory (G1 & K ~ BindCon d ty' T & G2) ->
+          K' # G1 & K ~ BindCon d ty' T & G2 ->
+          ok_env (G1 & K ~ BindCon d ty' T & G2) ->
+          contradictory (G1 & K' ~ BindCon d ty' T & map (Kbsubst K (FCon K')) G2).
 
     End PATCHECKPROPS.
 
@@ -143,6 +213,42 @@ Module TypingProps (P : PAT).
       Proof. introv Henv ; induction* Henv. Qed.
       #[export]
        Hint Resolve ok_env_ok : mcore.
+
+      Lemma ok_env_concat :
+        forall G1 G2,
+          ok_env (G1 & G2) ->
+          ok_env G1.
+      Proof with eauto.
+        introv Henv.
+        induction G2 using env_ind.
+        { Case "Empty". rew_env_concat in *... }
+        { Case "Push". apply IHG2. rew_env_concat in *.
+          inverts Henv ;
+            try (apply eq_push_inv in H; inverts H as []; substs~).
+          false. apply *empty_push_inv. }
+      Qed.
+
+      Lemma ok_type_ok_env :
+        forall Gamma T k,
+          Gamma |= T ~:: k ->
+          ok_env Gamma.
+      Proof.
+        introv hasType.
+        induction* hasType ; pick_fresh_gen L x; eauto using ok_env_concat.
+      Qed.
+      #[export]
+       Hint Resolve ok_type_ok_env : mcore.
+
+      Lemma ok_term_ok_env :
+        forall Gamma t T,
+          Gamma |= t ~: T ->
+          ok_env Gamma.
+      Proof.
+        introv hasType.
+        induction* hasType; pick_fresh_gen L x; eauto using ok_env_concat.
+      Qed.
+      #[export]
+       Hint Resolve ok_term_ok_env : mcore.
 
       Lemma ok_data_weakening :
         forall G3 G1 G2 d,
@@ -175,128 +281,17 @@ Module TypingProps (P : PAT).
           G1 & G3 |= T ~:: k ->
           ok_env (G1 & G2 & G3) ->
           G1 & G2 & G3 |= T ~:: k.
-      Proof.
+      Proof with eauto using ok_kind_weakening, ok_data_weakening with mcore.
         introv Htk Henv.
         remember (G1 & G3) as Gamma. gen G3.
-        induction* Htk; intros; substs.
-        { Case "TyFVar". constructors*. apply* binds_weaken. }
-        { Case "TyAll". apply_fresh* KAll. apply* ok_kind_weakening.
-          apply_ih_bind* H1.
-          constructor*. apply* ok_kind_weakening. }
-        { Case "TySem". constructors~.
+        induction Htk; intros; substs...
+        { Case "TyFVar". constructor~. apply* binds_weaken. }
+        { Case "TyAll". apply_fresh KAll...
+          apply_ih_bind H1 ; auto. constructor... }
+        { Case "TySem". constructor~.
           apply* Forall_pred_incl. intros p (ty1' & Hwf).
           eexists. apply* ok_pat_weakening. }
-        { Case "TyData". constructors*. apply* ok_data_weakening. }
-        { Case "TyDataSub". applys~ KDataSub d1. apply* ok_data_weakening. }
       Qed.
-
-      Lemma ok_env_ok_type :
-        forall Gamma x T,
-          ok_env Gamma ->
-          binds x (BindVar T) Gamma ->
-          Gamma |= T ~:: KiType.
-      Proof.
-        introv Henv Hbind.
-        induction* Henv ; try (binds_cases Hbind ; apply_empty* ok_type_weakening).
-        { Case "EnvEmpty". false. apply* binds_empty_inv. }
-        { Case "EnvVar". inverts* EQ. }
-      Qed.
-
-      Lemma ok_data_lcd : forall Gamma d, ok_data Gamma d -> lcd d.
-      Proof.
-        introv Hd. unfolds.
-        induction Hd ; rew_listx*. splits*. splits*.
-        induction H1 ; rew_listx*.
-      Qed.
-      #[export]
-       Hint Resolve ok_data_lcd : mcore.
-
-      Lemma ok_kind_lck : forall Gamma k, ok_kind Gamma k -> lck k.
-      Proof. introv Hk. destruct* Hk. Qed.
-      #[export]
-       Hint Resolve ok_kind_lck : mcore.
-
-      Lemma ok_type_lct :
-        forall Gamma T k,
-          Gamma |= T ~:: k ->
-          lct T.
-      Proof.
-        introv Htk ; induction* Htk.
-        - constructor~. apply* Forall_pred_incl.
-          intros p (ty1' & Hwf). apply* ok_pat_lcp.
-      Qed.
-      #[export]
-       Hint Resolve ok_type_lct : mcore.
-
-      Lemma ok_term_lct :
-        forall Gamma t T,
-          Gamma |= t ~: T ->
-          lct T.
-      Proof with eauto using ok_env_ok_type, ok_type_lct.
-        introv hasType.
-        induction* hasType...
-        { Case "TmLam". constructors...
-          pick_fresh_gen L y... }
-        { Case "TmApp". inverts* IHhasType1. }
-        { Case "TmTyLam". inverts* IHhasType.
-          assert(Hlct: lct ty2)...
-          pick_fresh X. rewrite *(tsubst_intro X).
-          apply* tsubst_lct. }
-        { Case "TmFix". inverts* IHhasType. }
-        { Case "TmProj1". inverts* IHhasType. }
-        { Case "TmProj2". inverts* IHhasType. }
-        { Case "TmType". pick_fresh T. applys~ H0 T. }
-        { Case "TmConDef". pick_fresh K. applys~ H3 K. }
-        { Case "TmSem". constructors...
-          pick_fresh_gen L y... forwards* Hpat : ok_pat_lcp. }
-        { Case "TmComp". inverts IHhasType1. inverts IHhasType2. constructor~. rew_listx~. }
-        { Case "TmSemApp". inverts* IHhasType1. }
-      Qed.
-      #[export]
-       Hint Resolve ok_term_lct : mcore.
-
-      Lemma ok_term_lc :
-        forall Gamma t T,
-          Gamma |= t ~: T ->
-          lc t.
-      Proof.
-        introv Htype; induction* Htype ; forwards* Hpat : ok_pat_lcp.
-      Qed.
-      #[export]
-       Hint Resolve ok_term_lc : mcore.
-
-      Lemma ok_env_push :
-        forall G1 x b,
-          ok_env (G1 & x ~ b) ->
-          ok_env G1.
-      Proof.
-        introv Henv. inverts Henv ;
-          try (apply eq_push_inv in H; inverts H as []; substs~).
-        false. apply *empty_push_inv.
-      Qed.
-
-      Lemma ok_type_ok_env :
-        forall Gamma T k,
-          Gamma |= T ~:: k ->
-          ok_env Gamma.
-      Proof.
-        introv hasType.
-        induction* hasType ; pick_fresh_gen L x; eauto using ok_env_push.
-      Qed.
-      #[export]
-       Hint Resolve ok_type_ok_env : mcore.
-
-      Lemma ok_term_ok_env :
-        forall Gamma t T,
-          Gamma |= t ~: T ->
-          ok_env Gamma.
-      Proof.
-        introv hasType.
-        induction* hasType; pick_fresh_gen L x;
-          eauto using ok_env_push.
-      Qed.
-      #[export]
-       Hint Resolve ok_term_ok_env : mcore.
 
       Lemma ok_term_weakening :
         forall G3 G2 G1 t T,
@@ -313,10 +308,17 @@ Module TypingProps (P : PAT).
           apply_ih_bind H1 ; auto. constructor... }
         { Case "TmCon". constructors...
           apply* binds_weaken. }
-        { Case "TmMatch". apply_fresh* TMatch as y...
-          + apply* ok_pat_weakening.
-          + apply_ih_bind H1 ; auto. constructor...
-            apply~ ok_type_weakening. apply* ok_pat_ok_type. }
+        { Case "TmMatch". apply_fresh TMatch ; intros...
+          - apply* ok_pat_weakening.
+          - do_rew_2 concat_assoc (applys H1 M) ; auto. easy.
+            constructor~.
+            + constructors~. apply* ok_pat_weakening.
+            + apply_empty ok_type_weakening.
+              * apply~ ok_type_weakening. apply* ok_pat_ok_type.
+              * constructors~. apply* ok_pat_weakening.
+          - apply_ih_bind (H3 y) ; auto.
+            constructors~. apply* ok_pat_weakening. }
+        { Case "TmNever". constructor... apply* contradictory_weakening. }
         { Case "TmType". apply_fresh TType as T...
           apply_ih_bind H0 ; auto. constructor... }
         { Case "TmConDef". apply_fresh TConDef as K...
@@ -329,49 +331,7 @@ Module TypingProps (P : PAT).
         { Case "TmSem". apply_fresh* TSem as y... apply* ok_pat_weakening.
           apply_ih_bind H2 ; auto. constructor...
           apply~ ok_type_weakening. apply* ok_pat_ok_type. }
-        { Case "TmSemApp". constructors~. apply~ pats_exhaustive_weakening. }
-      Qed.
-
-      Lemma ok_data_strengthening :
-        forall G1 G2 x T d,
-          ok_data (G1 & x ~ BindVar T & G2) d ->
-          ok_data (G1 & G2) d.
-      Proof.
-        introv Hd.
-        remember (G1 & x ~ BindVar T & G2) as Gamma.
-        induction Hd ; constructor*.
-        - substs ; binds_cases H0 ; auto.
-        - induction* H1 ; substs ; constructors*.
-          binds_cases H3 ; eauto.
-      Qed.
-
-      Lemma ok_kind_strengthening :
-        forall G1 G2 x T k,
-          ok_kind (G1 & x ~ BindVar T & G2) k ->
-          ok_kind (G1 & G2) k.
-      Proof.
-        introv Hk. remember (G1 & x ~ BindVar T & G2) as G.
-        destruct Hk ; substs*. constructor. apply* ok_data_strengthening.
-      Qed.
-
-      Lemma ok_type_strengthening :
-        forall G2 G1 x T1 T2 k,
-          G1 & x ~ BindVar T2 & G2 |= T1 ~:: k ->
-          ok_env (G1 & G2) ->
-          G1 & G2 |= T1 ~:: k.
-      Proof.
-        introv Htk. remember (G1 & x ~ BindVar T2 & G2) as G. gen G2.
-        induction Htk; intros; substs*.
-        { Case "TyFVar". constructors*.
-          binds_cases H0 ; auto. }
-        { Case "TyAll". apply_fresh* KAll as X.
-          apply* ok_kind_strengthening.
-          apply_ih_bind H1 ; eauto. constructor*. apply* ok_kind_strengthening. }
-        { Case "TySem". constructor~.
-          apply* Forall_pred_incl. intros p (ty1'&Hwf).
-          eexists. apply* ok_pat_strengthening. }
-        { Case "TyData". constructor~. apply* ok_data_strengthening. }
-        { Case "TyDataSub". applys~ KDataSub d1. apply* ok_data_strengthening. }
+        { Case "TmSemApp". constructors~. apply~ exhaustive_weakening. }
       Qed.
 
       Lemma ok_env_con_inv :
@@ -409,65 +369,334 @@ Module TypingProps (P : PAT).
         false. apply* empty_push_inv.
       Qed.
 
-      Lemma ok_env_strengthening :
-        forall G1 x T G3,
-          ok_env (G1 & x ~ BindVar T & G3) ->
-          ok_env (G1 & G3).
+      Lemma ok_env_binds_con_inv :
+        forall Gamma K d ty T,
+          ok_env Gamma  ->
+          binds K (BindCon d ty T) Gamma ->
+          exists L T',
+            T = FTName T'
+            /\ ok_data Gamma d
+            /\ (forall X, X \notin L -> Gamma & X ~ BindTVar (KiData d) |= {0 ~> TyFVar X}ty ~:: KiType)
+            /\ binds T' BindTName Gamma.
       Proof.
-        introv Henv. induction G3 using env_ind.
-        { Case "Empty". rewrite concat_empty_r in *. apply* ok_env_push. }
-        { Case "Push". rewrite concat_assoc in *.
-          specializes IHG3 (ok_env_push _ _ _ Henv).
-          lets [? Hdisj] : ok_push_inv (ok_env_ok _ Henv).
-          destruct v.
-          { SCase "BindTName". constructor~. }
-          { SCase "BindCon". forwards (L & T' & Heq & Hd & Htk & HT): ok_env_con_inv Henv.
-            substs. apply_fresh* EnvCon as K.
-            - apply* ok_data_strengthening.
-            - apply_ih_bind ok_type_strengthening ; eauto.
-              constructor~. constructor~. apply* ok_data_strengthening.
-            - binds_cases HT ; auto. }
-          { SCase "BindTVar". forwards Hk: ok_env_tvar_inv Henv.
-            constructor~. applys ok_kind_strengthening Hk. }
-          { SCase "BindVar". forwards Htk: ok_env_var_inv Henv.
-            constructor~. applys* ok_type_strengthening Htk. }
-          (* { SCase "BindMatch". constructor~. } *)
-        }
+        introv Henv Hbinds.
+        induction Gamma using env_ind.
+        - false. apply* binds_empty_inv.
+        - binds_cases Hbinds.
+          + destruct~ IHGamma as (L & T' & Heq & Hd & Htk & Hbinds'). apply* ok_env_concat.
+            exists (L \u dom Gamma \u \{x}) T'. splits*. apply_empty~ ok_data_weakening.
+            introv Hfresh. apply~ ok_type_weakening. constructor~. constructor.
+            apply_empty~ ok_data_weakening. apply* binds_concat_left_ok.
+          + inverts EQ. forwards* (L & T' & Heq & Hd & Htk & Hbinds') : ok_env_con_inv.
+            exists (L \u dom Gamma \u \{K}) T'. splits~. apply_empty~ ok_data_weakening.
+            introv Hfresh. apply~ ok_type_weakening. constructor~. constructor.
+            apply_empty~ ok_data_weakening. apply* binds_concat_left_ok.
       Qed.
 
-      Lemma ok_term_subst :
-        forall G2 G1 x T1 T2 t1 t2,
-          G1 & x ~ BindVar T2 & G2 |= t1 ~: T1 ->
-          G1 |= t2 ~: T2 ->
-          G1 & G2 |= [x => t2]t1 ~: T1.
-      Proof with eauto using ok_data_strengthening, ok_kind_strengthening,
-          ok_type_strengthening, ok_env_strengthening with mcore.
-        introv hasType1 hasType2.
-        remember (G1 & x ~ BindVar T2 & G2) as G. gen G2.
-        induction hasType1; intros; simpls; substs...
-        { Case "TmFVar". solve_var.
-          - binds_get H0... apply_empty ok_term_weakening...
-          - binds_cases H0... }
-        { Case "TmLam". apply_fresh* TLam as y...
-          rewrite subst_open_comm... apply_ih_bind* H1. }
-        { Case "TmTyLam". apply_fresh* TTyLam as X...
-          rewrite* topen_t_subst_comm. apply_ih_bind* H1. }
-        { Case "TmTyApp". constructors... }
-        { Case "TmCon". constructors... binds_cases H ; auto. }
-        { Case "TmMatch". apply_fresh* TMatch as y...
-          - apply* ok_pat_strengthening.
-          - rewrite subst_open_comm... apply_ih_bind* H1. }
-        { Case "TmType". apply_fresh* TType as T...
-          rewrite* Topen_t_subst_comm. apply_ih_bind* H0. }
-        { Case "TmConDef". apply_fresh* TConDef as K...
-          - apply_ih_bind ok_type_strengthening ; eauto. constructor...
-          - binds_cases H1; auto.
-          - rewrite* Kopen_t_subst_comm. apply_ih_bind* H3. }
-        { Case "TmSem". apply_fresh* TSem as y...
-          - apply* ok_pat_strengthening.
-          - rewrite subst_open_comm... apply_ih_bind* H2. }
-        { Case "TmSemApp". constructors~.
-          apply* pats_exhaustive_strengthening. }
+      Lemma ok_env_binds_tvar_inv :
+        forall Gamma X k,
+          ok_env Gamma ->
+          binds X (BindTVar k) Gamma ->
+          ok_kind Gamma k.
+      Proof.
+        introv Henv Hbinds.
+        induction Gamma using env_ind.
+        - false. apply* binds_empty_inv.
+        - binds_cases Hbinds.
+          + apply_empty~ ok_kind_weakening. apply~ IHGamma. apply* ok_env_concat.
+          + substs. forwards* Hk: ok_env_tvar_inv. apply_empty~ ok_kind_weakening.
+      Qed.
+
+      Lemma ok_env_binds_var_inv :
+        forall Gamma x ty,
+          ok_env Gamma ->
+          binds x (BindVar ty) Gamma ->
+          Gamma |= ty ~:: KiType.
+      Proof.
+        introv Henv Hbinds.
+        induction Gamma using env_ind.
+          - false. apply* binds_empty_inv.
+          - binds_cases Hbinds.
+            + apply_empty~ ok_type_weakening. forwards~ ?: ok_env_concat Henv.
+            + inverts EQ. apply_empty~ ok_type_weakening. apply* ok_env_var_inv.
+      Qed.
+
+      Lemma ok_data_lcd : forall Gamma d, ok_data Gamma d -> lcd d.
+      Proof.
+        introv Hd. unfolds.
+        induction Hd ; rew_listx*. splits*. splits*.
+        induction H1 ; rew_listx*.
+      Qed.
+      #[export]
+       Hint Resolve ok_data_lcd : mcore.
+
+      Lemma ok_kind_lck : forall Gamma k, ok_kind Gamma k -> lck k.
+      Proof. introv Hk. destruct* Hk. Qed.
+      #[export]
+       Hint Resolve ok_kind_lck : mcore.
+
+      Lemma ok_type_lct :
+        forall Gamma T k,
+          Gamma |= T ~:: k ->
+          lct T.
+      Proof.
+        introv Htk ; induction* Htk.
+        - constructor~. apply* Forall_pred_incl.
+          intros p (ty1' & Hwf). apply* ok_pat_lcp.
+      Qed.
+      #[export]
+       Hint Resolve ok_type_lct : mcore.
+
+      Lemma ok_term_lct :
+        forall Gamma t T,
+          Gamma |= t ~: T ->
+          lct T.
+      Proof with eauto using ok_env_binds_var_inv, ok_type_lct.
+        introv hasType.
+        induction* hasType...
+        { Case "TmLam". constructors...
+          pick_fresh_gen L y... }
+        { Case "TmApp". inverts* IHhasType1. }
+        { Case "TmTyLam". inverts* IHhasType.
+          assert(Hlct: lct ty2)...
+          pick_fresh X. rewrite *(tsubst_intro X).
+          apply* tsubst_lct. }
+        { Case "TmFix". inverts* IHhasType. }
+        { Case "TmProj1". inverts* IHhasType. }
+        { Case "TmProj2". inverts* IHhasType. }
+        { Case "TmMatch". pick_fresh_gen L y... }
+        { Case "TmType". pick_fresh T. applys~ H0 T. }
+        { Case "TmConDef". pick_fresh K. applys~ H3 K. }
+        { Case "TmSem". constructors...
+          pick_fresh_gen L y... forwards* Hpat : ok_pat_lcp. }
+        { Case "TmComp". inverts IHhasType1. inverts IHhasType2. constructor~. rew_listx~. }
+        { Case "TmSemApp". inverts* IHhasType1. }
+      Qed.
+      #[export]
+       Hint Resolve ok_term_lct : mcore.
+
+      Lemma ok_term_lc :
+        forall Gamma t T,
+          Gamma |= t ~: T ->
+          lc t.
+      Proof.
+        introv Htype; induction* Htype.
+        - pick_fresh_gen L y. forwards* Hpat : ok_pat_lcp.
+        - forwards* Hpat : ok_pat_lcp.
+      Qed.
+      #[export]
+       Hint Resolve ok_term_lc : mcore.
+
+      Lemma ok_type_ok_kind :
+        forall Gamma T k,
+          Gamma |= T ~:: k ->
+          ok_kind Gamma k.
+      Proof. introv Htk. induction* Htk. apply* ok_env_binds_tvar_inv. Qed.
+
+      Lemma ok_data_notin_T :
+        forall Gamma d X,
+          ok_data Gamma d ->
+          X # Gamma ->
+          X \notin Tfv_d d.
+      Proof.
+        introv Hd Hfresh. unfolds Tfv_d.
+        induction Hd ; rew_listx ; simpls~.
+        rewrite notin_union. splits*.
+        - rewrite notin_singleton. intro. substs.
+          forwards~ Hin : get_some_inv H0.
+      Qed.
+
+      Lemma ok_kind_notin_T :
+        forall Gamma k X,
+          ok_kind Gamma k ->
+          X # Gamma ->
+          X \notin Tfv_k k.
+      Proof.
+        introv Hk Hfresh. unfolds Tfv_k.
+        destruct~ Hk. apply* ok_data_notin_T.
+      Qed.
+
+      Lemma assoc_data_in :
+        forall d T Ks,
+          mem (FTName T, Ks) d -> T \in Tfv_d d.
+      Proof.
+        introv Hassoc. unfolds Tfv_d.
+        induction Hassoc ; rew_listx ; simpls~.
+        - rewrite~ in_union. rewrite~ in_singleton.
+        - destruct y. rewrite~ in_union.
+      Qed.
+
+      Lemma ok_type_notin_T :
+        forall Gamma T k X,
+          Gamma |= T ~:: k ->
+          X # Gamma ->
+          X \notin Tfv_ty T.
+      Proof with eauto using ok_data_notin_T, ok_kind_notin_T.
+        introv Htk Hfresh.
+        induction Htk; simpls...
+        { Case "TyAll". rewrite notin_union. splits...
+          pick_fresh Y. forwards~ Htk: H1 Y.
+          rewrite topen_notin_T in Htk ; simpls~. }
+        { Case "TyCon". rewrite notin_union. splits~.
+          forwards Hk: ok_type_ok_kind Htk.
+          forwards~ Hnin : ok_kind_notin_T X Hk.
+          assert (X <> T) by (intro ; substs ; apply Hnin ; applys* assoc_data_in).
+          auto. }
+      Qed.
+
+      Lemma ok_term_notin_T :
+        forall Gamma t T X,
+          Gamma |= t ~: T ->
+          X # Gamma ->
+          X \notin Tfv_t t.
+      Proof with eauto using ok_data_notin_T, ok_kind_notin_T, ok_type_notin_T.
+        introv Htype Hfresh.
+        induction Htype; simpls ; rewrite_all notin_union...
+        - pick_fresh x. forwards~ Hnin : H1 x. rewrite open_notin_T in Hnin...
+        - pick_fresh Y. forwards~ Hnin : H1 Y. rewrite topen_t_notin_T in Hnin...
+        - pick_fresh M. pick_fresh x. forwards~ Hnin1 : H1 M x.
+          forwards~ Hnin2 : H3 M. rewrite open_notin_T in Hnin1...
+        - pick_fresh T. forwards~ Hnin : Topen_t_notin_T (H0 T).
+        - pick_fresh K. forwards~ Hnin1 : Kopen_t_notin_T (H3 K).
+          forwards~ Hnin2 : ok_type_notin_T X (H0 K).
+          rewrite topen_notin_T in Hnin2 ; simpls~.
+          assert (X <> T)... intro ; substs. forwards~ ?: get_some_inv H1.
+        - pick_fresh x. forwards~ Hnin : H2 x. rewrite open_notin_T in Hnin...
+      Qed.
+
+      Lemma data_sub_notin_T :
+        forall T d1 d2,
+          T \notin Tfv_d d1 ->
+          data_sub d2 d1 ->
+          T \notin Tfv_d d2.
+      Proof with eauto.
+        introv Hnin Hsub. unfolds data_sub. unfolds Tfv_d.
+        induction d2 ; rew_listx ; simpls~.
+        rewrite notin_union ; split~. destruct a. destruct~ t.
+        assert (T <> v)... intro ; substs.
+        forwards~ (?&Hmem&?) : Hsub. forwards~ (?&?&Heq) : mem_inv_middle Hmem.
+        substs. rew_listx* in Hnin. simpls.
+        notin_false.
+      Qed.
+
+      Lemma ok_data_notin_K :
+        forall Gamma d X,
+          ok_data Gamma d ->
+          X # Gamma ->
+          X \notin Kfv_d d.
+      Proof.
+        introv Hd Hfresh. unfolds Kfv_d.
+        induction Hd ; rew_listx ; simpls~.
+        rewrite notin_union. splits*.
+        induction H1 ; rew_listx ; simpls~ ; rewrite notin_union ; splits~.
+        - rewrite notin_singleton. intro. substs.
+          forwards~ Hin : get_some_inv H3.
+      Qed.
+
+      Lemma ok_kind_notin_K :
+        forall Gamma k X,
+          ok_kind Gamma k ->
+          X # Gamma ->
+          X \notin Kfv_k k.
+      Proof.
+        introv Hk Hfresh. unfolds Kfv_k.
+        destruct~ Hk. apply* ok_data_notin_K.
+      Qed.
+
+      Lemma ok_type_notin_K :
+        forall Gamma T k X,
+          Gamma |= T ~:: k ->
+          X # Gamma ->
+          X \notin Kfv_ty T.
+      Proof with eauto using ok_data_notin_K, ok_kind_notin_K, ok_pat_notin_K.
+        introv Htk Hfresh.
+        induction Htk; simpls...
+        { Case "TyAll". rewrite notin_union. splits...
+          pick_fresh Y. forwards~ Htk: H1 Y.
+          rewrite topen_notin_K in Htk ; simpls~. }
+        { Case "TySem". rewrite_all notin_union. repeat split~.
+          induction ps ; rew_listx ; simpls~. rew_listx in H. destruct H as ((ty1'&Hfw)&?).
+          rewrite notin_union... }
+      Qed.
+
+      Lemma ok_term_notin_K :
+        forall Gamma t T X,
+          Gamma |= t ~: T ->
+          X # Gamma ->
+          X \notin Kfv_t t.
+      Proof with eauto using ok_data_notin_K, ok_kind_notin_K, ok_type_notin_K, ok_pat_notin_K.
+        introv Htype Hfresh.
+        induction Htype; simpls ; rewrite_all notin_union...
+        - pick_fresh x. forwards~ Hnin : H1 x. rewrite open_notin_K in Hnin...
+        - pick_fresh Y. forwards~ Hnin : H1 Y. rewrite topen_t_notin_K in Hnin...
+        - assert (X <> K)... intro ; substs. forwards~ ?: get_some_inv H.
+        - pick_fresh M. pick_fresh x. forwards~ Hnin1 : H1 M x.
+          forwards~ Hnin2 : H3 M. rewrite open_notin_K in Hnin1...
+        - pick_fresh T. forwards~ Hnin : Topen_t_notin_K (H0 T).
+        - pick_fresh K0. forwards~ Hnin1 : Kopen_t_notin_K (H3 K0).
+          forwards~ Hnin2 : ok_type_notin_K X (H0 K0).
+          rewrite topen_notin_K in Hnin2 ; simpls...
+        - pick_fresh x. forwards~ Hnin1 : H2 x. rewrite open_notin_K in Hnin1...
+      Qed.
+
+      Lemma data_sub_notin_K :
+        forall K d1 d2,
+          K \notin Kfv_d d1 ->
+          data_sub d2 d1 ->
+          K \notin Kfv_d d2.
+      Proof with eauto.
+        introv Hnin Hsub. unfolds data_sub. unfolds Kfv_d.
+        induction d2 ; rew_listx ; simpls~.
+        rewrite notin_union ; split~. destruct a.
+        forwards* (Ks'&Hmem&HsubK) : Hsub.
+        forwards~ (?&?&Heq) : mem_inv_middle Hmem. substs.
+        rew_listx* in Hnin ; simpls.
+        assert (HninK : K \notin fold varsM (fun K => Kfv K) Ks')...
+        clears IHd2 Hsub Hnin Hmem.
+        induction l ; rew_listx ; simpls~.
+        rewrite notin_union ; split~. destruct~ a.
+        assert (K <> v)... intro ; substs.
+        forwards~ Hmem : HsubK.
+        forwards~ (?&?&Heq) : mem_inv_middle Hmem. substs.
+        rew_listx* in HninK. simpls. notin_false.
+      Qed.
+
+      Lemma ok_data_strengthening :
+        forall G1 G2 x T d,
+          ok_data (G1 & x ~ BindVar T & G2) d ->
+          ok_data (G1 & G2) d.
+      Proof.
+        introv Hd.
+        remember (G1 & x ~ BindVar T & G2) as Gamma.
+        induction Hd ; constructor*.
+        - substs ; binds_cases H0 ; auto.
+        - induction* H1 ; substs ; constructors*.
+          binds_cases H3 ; eauto.
+      Qed.
+
+      Lemma ok_kind_strengthening :
+        forall G1 G2 x T k,
+          ok_kind (G1 & x ~ BindVar T & G2) k ->
+          ok_kind (G1 & G2) k.
+      Proof.
+        introv Hk. remember (G1 & x ~ BindVar T & G2) as G.
+        destruct Hk ; substs*. constructor. apply* ok_data_strengthening.
+      Qed.
+
+      Lemma ok_type_strengthening :
+        forall G2 G1 x T1 T2 k,
+          G1 & x ~ BindVar T2 & G2 |= T1 ~:: k ->
+          ok_env (G1 & G2) ->
+          G1 & G2 |= T1 ~:: k.
+      Proof with eauto using ok_data_strengthening, ok_kind_strengthening with mcore.
+        introv Htk. remember (G1 & x ~ BindVar T2 & G2). gen G2.
+        induction Htk; intros; substs...
+        { Case "TyFVar". constructor~. binds_cases H0 ; auto. }
+        { Case "TyAll". apply_fresh KAll as X...
+          apply_ih_bind H1 ; eauto. constructor... }
+        { Case "TySem". constructor~.
+          apply* Forall_pred_incl. intros p (ty1'&Hwf).
+          eexists. apply* ok_pat_strengthening. }
       Qed.
 
       Lemma ok_data_tvar_strengthening :
@@ -483,21 +712,6 @@ Module TypingProps (P : PAT).
           binds_cases H3 ; eauto.
       Qed.
 
-      Lemma ok_data_bsubst :
-        forall G1 G2 X T d,
-          ok_data (G1 & G2) d ->
-          ok_data (G1 & map (bsubst X T) G2) d.
-      Proof.
-        introv Hd.
-        remember (G1 & G2) as Gamma.
-        induction Hd ; constructor*.
-        - substs ; binds_cases H0 ; auto.
-          replaces BindTName with (bsubst X T BindTName) ; auto.
-        - induction* H1 ; substs.
-          binds_cases H3 ; constructors*.
-          replaces (BindCon d0 ({X => T} ty) T1) with (bsubst X T (BindCon d0 ty T1)) ; auto.
-      Qed.
-
       Lemma ok_kind_tvar_strengthening :
         forall G1 G2 x k' k,
           ok_kind (G1 & x ~ BindTVar k' & G2) k ->
@@ -505,6 +719,229 @@ Module TypingProps (P : PAT).
       Proof.
         introv Hk. remember (G1 & x ~ BindTVar k' & G2) as Gamma.
         destruct* Hk. constructor. substs. apply* ok_data_tvar_strengthening.
+      Qed.
+
+      Lemma ok_data_match_strengthening :
+        forall G2 G1 M t p m d,
+          ok_data (G1 & M ~ BindMatch t p m & G2) d ->
+          ok_data (G1 & G2) d.
+      Proof.
+        introv Hd. remember (G1 & M ~ BindMatch t p m & G2).
+        induction Hd ; constructor~.
+        - substs ; binds_cases H0 ; auto.
+        - induction H1 ; substs ; constructors*.
+          binds_cases H3 ; eauto.
+      Qed.
+
+      Lemma ok_kind_match_strengthening :
+        forall G2 G1 M t p m k,
+          ok_kind (G1 & M ~ BindMatch t p m & G2) k ->
+          ok_kind (G1 & G2) k.
+      Proof.
+        introv Hk. remember (G1 & M ~ BindMatch t p m & G2).
+        destruct* Hk. constructor. substs. apply* ok_data_match_strengthening.
+      Qed.
+
+      Lemma ok_type_match_strengthening :
+        forall G2 G1 M t p m T k,
+          G1 & M ~ BindMatch t p m & G2 |= T ~:: k ->
+          ok_env (G1 & G2) ->
+          G1 & G2 |= T ~:: k.
+      Proof with eauto using ok_data_match_strengthening, ok_kind_match_strengthening with mcore.
+        introv Htk.
+        remember (G1 & M ~ BindMatch t p m & G2). gen G2.
+        induction Htk; intros; substs...
+        { Case "TyFVar". constructor~. binds_cases H0 ; auto. }
+        { Case "TyAll". apply_fresh KAll as X...
+          apply_ih_bind H1 ; eauto. constructor... }
+        { Case "TySem". constructor~.
+          apply* Forall_pred_incl. intros p' (ty1'&Hwf).
+          eexists. apply* ok_pat_match_strengthening. }
+      Qed.
+
+      Lemma ok_data_tname_strengthening :
+        forall G2 G1 T d,
+          T \notin Tfv_d d ->
+          ok_data (G1 & T ~ BindTName & G2) d ->
+          ok_data (G1 & G2) d.
+      Proof.
+        introv Hfv Hd. remember (G1 & T ~ BindTName & G2) as Gamma eqn:HGamma.
+        unfolds Tfv_d. induction Hd ; substs ; constructor ; rew_listx in Hfv ; simpls~.
+        - binds_cases H0 ; auto. notin_false.
+        - induction* Ks. inverts H1.
+          constructors~. binds_cases H8 ; eauto.
+      Qed.
+
+      Lemma ok_kind_tname_strengthening :
+        forall T G2 G1 k,
+          T \notin Tfv_k k ->
+          ok_kind (G1 & T ~ BindTName & G2) k ->
+          ok_kind (G1 & G2) k.
+      Proof with eauto using ok_data_tname_strengthening with mcore.
+        introv Hfv Hk.
+        remember (G1 & T ~ BindTName & G2) as Gamma eqn:HGamma.
+        induction Hk ; substs...
+      Qed.
+
+      Lemma ok_type_tname_strengthening :
+        forall T G2 G1 ty k,
+          T \notin Tfv_ty ty ->
+          G1 & T ~ BindTName & G2 |= ty ~:: k ->
+          ok_env (G1 & G2) ->
+          G1 & G2 |= ty ~:: k.
+      Proof with eauto using ok_data_tname_strengthening, ok_kind_tname_strengthening with mcore.
+        introv Hfv Htk Henv.
+        remember (G1 & T ~ BindTName & G2) as Gamma eqn:HGamma. gen G2.
+        induction Htk ; intros ; simpls ; substs...
+        { Case "TyFVar". constructor~. binds_cases H0 ; auto. }
+        { Case "TyAll". rewrite notin_union in Hfv ; destruct Hfv.
+          apply_fresh KAll as X...
+          apply_ih_bind H1 ; auto. rewrite topen_notin_T ; simpls~. constructors... }
+        { Case "TySem". constructor~. apply* Forall_pred_incl.
+          intros p (ty1'&Hwf). eexists. apply* ok_pat_tname_strengthening ; auto. }
+        { Case "TyDataSub". applys~ KDataSub d1.
+          apply* ok_data_tname_strengthening.
+          forwards~ Hd1 : IHHtk. forwards Hk : ok_type_ok_kind Hd1.
+          inverts Hk. forwards~ Hnin : ok_data_notin_T T H3.
+          forwards* (Hfr1&Hfr2) : ok_middle_inv G1 G2.
+          apply* data_sub_notin_T. }
+      Qed.
+
+      Lemma ok_data_con_strengthening :
+        forall K G2 G1 d' ty' T d,
+          K \notin Kfv_d d ->
+          ok_data (G1 & K ~ BindCon d' ty' T & G2) d ->
+          ok_data (G1 & G2) d.
+      Proof.
+        introv Hfv Hd. remember (G1 & K ~ BindCon d' ty' T & G2) as Gamma eqn:HGamma.
+        unfolds Kfv_d. induction Hd ; substs ; constructor ; rew_listx in Hfv ; simpls~.
+        - binds_cases H0 ; auto.
+        - induction* Ks. inverts H1. rew_listx in Hfv ; simpls~.
+          constructors~. binds_cases H8 ; eauto. notin_false.
+      Qed.
+
+      Lemma ok_kind_con_strengthening :
+        forall K G2 G1 d ty' T k,
+          K \notin Kfv_k k ->
+          ok_kind (G1 & K ~ BindCon d ty' T & G2) k ->
+          ok_kind (G1 & G2) k.
+      Proof with eauto using ok_data_con_strengthening with mcore.
+        introv Hfv Hk.
+        remember (G1 & K ~ BindCon d ty' T & G2) as Gamma eqn:HGamma.
+        induction Hk ; substs...
+      Qed.
+
+      Lemma ok_type_con_strengthening :
+        forall K G2 G1 d ty' T ty k,
+          K \notin Kfv_ty ty ->
+          G1 & K ~ BindCon d ty' T & G2 |= ty ~:: k ->
+          ok_env (G1 & G2) ->
+          G1 & G2 |= ty ~:: k.
+      Proof with eauto using ok_data_con_strengthening, ok_kind_con_strengthening with mcore.
+        introv Hfv Htk Henv.
+        remember (G1 & K ~ BindCon d ty' T & G2) as Gamma eqn:HGamma. gen G2.
+        induction Htk ; intros ; simpls ; substs...
+        { Case "TyFVar". constructor~. binds_cases H0 ; auto. }
+        { Case "TyAll". rewrite notin_union in Hfv ; destruct Hfv.
+          apply_fresh KAll as X...
+          apply_ih_bind H1 ; auto. rewrite topen_notin_K ; simpls~. constructors... }
+        { Case "TySem". constructor~. apply* Forall_pred_incl.
+          intros p (ty1'&Hwf). eexists. apply* ok_pat_con_strengthening ; auto. }
+        { Case "TyDataSub". applys~ KDataSub d1.
+          apply* ok_data_con_strengthening.
+          forwards~ Hd1 : IHHtk. forwards Hk : ok_type_ok_kind Hd1.
+          inverts Hk. forwards~ Hnin : ok_data_notin_K K H3.
+          forwards* (Hfr1&Hfr2) : ok_middle_inv G1 G2.
+          apply* data_sub_notin_K. }
+      Qed.
+
+      Lemma ok_data_tbsubst :
+        forall G1 G2 X T d,
+          ok_data (G1 & G2) d ->
+          ok_data (G1 & map (tbsubst X T) G2) d.
+      Proof.
+        introv Hd.
+        remember (G1 & G2) as Gamma.
+        induction Hd ; constructor*.
+        - substs ; binds_cases H0 ; auto.
+          replaces BindTName with (tbsubst X T BindTName) ; auto.
+        - induction* H1 ; substs.
+          binds_cases H3 ; constructors*.
+          replaces (BindCon d0 ({X => T} ty) T1) with (tbsubst X T (BindCon d0 ty T1)) ; auto.
+      Qed.
+
+      Lemma ok_kind_tbsubst :
+        forall G1 G2 X T k,
+          ok_kind (G1 & G2) k ->
+          ok_kind (G1 & map (tbsubst X T) G2) k.
+      Proof.
+        introv Hk. remember (G1 & G2) as Gamma.
+        destruct* Hk. constructor. substs. apply* ok_data_tbsubst.
+      Qed.
+
+      Lemma ok_type_tsubst :
+        forall G2 G1 X T1 T2 k k',
+          G1 & X ~ BindTVar k' & G2 |= T1 ~:: k ->
+          G1 |= T2 ~:: k' ->
+          ok_env (G1 & map (tbsubst X T2) G2) ->
+          G1 & map (tbsubst X T2) G2 |= {X => T2} T1 ~:: k.
+      Proof with eauto using ok_data_tbsubst, ok_kind_tbsubst, ok_type_lct,
+          ok_data_tvar_strengthening, ok_kind_tvar_strengthening with mcore.
+        introv Htk1 Htk2 Henv.
+        remember (G1 & X ~ BindTVar k' & G2) as G. gen G2.
+        induction Htk1; intros; substs; simpls...
+        { Case "TyFVar". solve_var.
+          + binds_get H0. lets* [Hok ?] : ok_concat_inv (ok_env_ok _ Henv).
+            apply_empty* ok_type_weakening.
+          + constructors~. binds_cases H0...
+            replaces (BindTVar k) with (tbsubst X T2 (BindTVar k))... }
+        { Case "TyAll". apply_fresh KAll... rewrite tsubst_topen_comm...
+          replaces (BindTVar k) with (tbsubst X T2 (BindTVar k))...
+          apply_ih_map_bind H1 ; auto. constructor... }
+        { Case "TySem". constructor~. apply* Forall_pred_incl.
+          intros p (ty1'&Hwf). eexists. apply* ok_pat_tsubst. }
+      Qed.
+
+      Lemma ok_term_ok_type :
+        forall Gamma t ty,
+          Gamma |= t ~: ty ->
+          Gamma |= ty ~:: KiType.
+      Proof with eauto with mcore.
+        introv Htype.
+        induction* Htype.
+        { Case "TmFVar". apply* ok_env_binds_var_inv. }
+        { Case "TmLam". constructor~. pick_fresh x. forwards~ Htk : H1 x.
+          apply_empty* ok_type_strengthening. }
+        { Case "TmApp". inverts~ IHHtype1. }
+        { Case "TmTyLam". inverts IHHtype. pick_fresh X. rewrite~ (tsubst_intro X).
+          apply_empty* ok_type_tsubst. }
+        { Case "TmFix". inverts~ IHHtype. }
+        { Case "TmProj1". inverts~ IHHtype. }
+        { Case "TmProj2". inverts~ IHHtype. }
+        { Case "TmMatch". pick_fresh M. pick_fresh x. forwards~ Htk : H1 M x.
+          apply_empty* ok_type_match_strengthening. apply_empty ok_type_strengthening... }
+        { Case "TmType". pick_fresh T. apply_empty* (ok_type_tname_strengthening T). }
+        { Case "TmConDef". pick_fresh K. apply_empty* (ok_type_con_strengthening K). }
+        { Case "TmSem". constructor ; rew_listx*.
+          pick_fresh x. forwards~ Htk : H2 x.
+          apply_empty* ok_type_strengthening. }
+        { Case "TmComp". inverts IHHtype1. inverts IHHtype2. constructor ; rew_listx~. }
+        { Case "TmSemApp". inverts~ IHHtype1. }
+      Qed.
+
+      Lemma ok_data_bsubst :
+        forall G1 G2 x t d,
+          ok_data (G1 & G2) d ->
+          ok_data (G1 & map (bsubst x t) G2) d.
+      Proof.
+        introv Hd.
+        remember (G1 & G2) as Gamma.
+        induction Hd ; constructor*.
+        - substs ; binds_cases H0 ; auto.
+          replaces BindTName with (bsubst x t BindTName) ; auto.
+        - induction* H1 ; substs.
+          binds_cases H3 ; constructors*.
+          replaces (BindCon d0 ty T0) with (bsubst x t (BindCon d0 ty T0)) ; auto.
       Qed.
 
       Lemma ok_kind_bsubst :
@@ -516,70 +953,88 @@ Module TypingProps (P : PAT).
         destruct* Hk. constructor. substs. apply* ok_data_bsubst.
       Qed.
 
-      Lemma ok_type_tsubst :
-        forall G2 G1 X T1 T2 k k',
-          G1 & X ~ BindTVar k' & G2 |= T1 ~:: k ->
-          G1 |= T2 ~:: k' ->
-          ok_env (G1 & map (bsubst X T2) G2) ->
-          G1 & map (bsubst X T2) G2 |= {X => T2} T1 ~:: k.
-      Proof with eauto using ok_data_bsubst, ok_kind_bsubst, ok_type_lct,
-          ok_data_tvar_strengthening, ok_kind_tvar_strengthening with mcore.
-        introv Htk1 Htk2 Henv.
-        remember (G1 & X ~ BindTVar k' & G2) as G. gen G2.
-        induction Htk1; intros; substs; simpls...
-        { Case "TyFVar". solve_var.
-          + binds_get H0. lets* [Hok ?] : ok_concat_inv (ok_env_ok _ Henv).
-            apply_empty* ok_type_weakening.
-          + constructors~. binds_cases H0...
-            replaces (BindTVar k) with (bsubst X T2 (BindTVar k))... }
-        { Case "TyAll". apply_fresh KAll... rewrite tsubst_topen_comm...
-          replaces (BindTVar k) with (bsubst X T2 (BindTVar k))...
+      Lemma ok_type_subst :
+        forall G2 G1 x t T1 T2 k,
+          G1 & x ~ BindVar T2 & G2 |= T1 ~:: k ->
+          ok_env (G1 & map (bsubst x t) G2) ->
+          G1 & map (bsubst x t) G2 |= T1 ~:: k.
+      Proof with eauto using ok_data_bsubst, ok_kind_bsubst,
+          ok_data_strengthening, ok_kind_strengthening with mcore.
+        introv Htk. remember (G1 & x ~ BindVar T2 & G2) as G. gen G2.
+        induction Htk; intros; substs; simpls...
+        { Case "TyFVar". constructor~. binds_cases H0 ; auto.
+          replaces (BindTVar k) with (bsubst x t (BindTVar k))... }
+        { Case "TyAll". apply_fresh KAll...
+          replaces (BindTVar k) with (bsubst x t (BindTVar k))...
           apply_ih_map_bind H1 ; auto. constructor... }
         { Case "TySem". constructor~. apply* Forall_pred_incl.
-          intros p (ty1'&Hwf). eexists. apply* ok_pat_tsubst. }
+          intros p (ty1'&Hwf). eexists.
+          apply ok_pat_bsubst. apply* ok_pat_strengthening. }
       Qed.
 
-      Lemma bsubst_ok_env :
-        forall G1 G2 X T2 k,
-          G1 |= T2 ~:: k ->
-          ok_env (G1 & X ~ BindTVar k & G2) ->
-          ok_env (G1 & map (bsubst X T2) G2).
-      Proof with eauto using ok_data_bsubst, ok_kind_bsubst, ok_type_lct,
-          ok_data_tvar_strengthening, ok_kind_tvar_strengthening with mcore.
-        introv Htk Henv.
-        induction G2 using env_ind.
-        { Case "Empty". autorewrite with rew_env_map rew_env_concat in *.
-          apply* ok_env_push. }
-        { Case "Push". autorewrite with rew_env_map rew_env_concat in *.
-          specializes IHG2 (ok_env_push _ _ _ Henv).
-          lets [? Hdisj] : ok_push_inv (ok_env_ok _ Henv).
-          destruct v.
-          { SCase "BindTName". constructor~. }
-          { SCase "BindCon". forwards (L & T' & Heq & Hd & Htk' & HT): ok_env_con_inv Henv.
-            substs. apply_fresh EnvCon as K...
-            - replaces (BindTVar (KiData d)) with (bsubst X T2 (BindTVar (KiData d))) ; auto.
-              rewrite tsubst_topen_comm...
-              apply_ih_map_bind ok_type_tsubst ; try rewrite* concat_assoc ; auto.
-              constructor~. constructor...
-            - binds_cases HT ; auto.
-              replaces BindTName with (bsubst X T2 BindTName) ; auto. }
-          { SCase "BindTVar". forwards Hk: ok_env_tvar_inv Henv. constructor... }
-          { SCase "BindVar". forwards Htk': ok_env_var_inv Henv.
-            constructor~. applys* ok_type_tsubst Htk'. }
-          (* { SCase "BindMatch". constructor~. } *)
-        }
-      Qed.
-
-      Lemma ok_env_concat :
-        forall G1 G2,
-          ok_env (G1 & G2) ->
-          ok_env G1.
-      Proof with eauto.
-        introv Henv.
-        induction G2 using env_ind.
-        { Case "Empty". rew_env_concat in *... }
-        { Case "Push". apply IHG2. rew_env_concat in *.
-          apply* ok_env_push. }
+      Lemma ok_term_subst :
+        forall G2 G1 x t1 t2 T1 T2,
+          G1 & x ~ BindVar T2 & G2 |= t1 ~: T1 ->
+          G1 |= t2 ~: T2 ->
+          ok_env (G1 & map (bsubst x t2) G2) ->
+          G1 & map (bsubst x t2) G2 |= [x => t2]t1 ~: T1.
+      Proof with eauto using ok_data_strengthening, ok_kind_strengthening,
+          ok_data_bsubst, ok_kind_bsubst, ok_type_subst with mcore.
+        introv Htype1 Htype2.
+        remember (G1 & x ~ BindVar T2 & G2). gen G2.
+        induction Htype1 ; intros ; simpls ; substs...
+        { Case "TmFVar". cases_if.
+          - binds_get H0... apply_empty ok_term_weakening ; auto.
+          - binds_cases H0... constructor ; auto.
+            replaces (BindVar ty) with (bsubst x t2 (BindVar ty))... }
+        { Case "TmLam". apply_fresh TLam as y...
+          replaces (BindVar ty1) with (bsubst x t2 (BindVar ty1))...
+          rewrite subst_open_comm... apply_ih_map_bind H1 ; auto.
+          constructor... }
+        { Case "TmTyLam". apply_fresh* TTyLam as X... rewrite* topen_t_subst_comm.
+          replaces (BindTVar k) with (bsubst x t2 (BindTVar k))...
+          apply_ih_map_bind H1 ; auto. constructor... }
+        { Case "TmCon". constructors... binds_cases H ; auto.
+          replaces (BindCon d ty1 (FTName T))
+            with (bsubst x t2 (BindCon d ty1 (FTName T)))... }
+        { Case "TmMatch". apply_fresh TMatch ; intros...
+          - apply ok_pat_bsubst. apply* ok_pat_strengthening.
+          - replaces (BindVar ty1') with (bsubst x t2 (BindVar ty1'))...
+            replaces (BindMatch ([x => t2]t) p true) with (bsubst x t2 (BindMatch t p true))...
+            rewrite subst_open_comm...
+            do_rew_2 concat_assoc_map_push (applys H1 M) ; auto. rewrite_all~ concat_assoc.
+            constructor~.
+            + constructors... apply ok_pat_bsubst. apply* ok_pat_strengthening.
+            + apply_ih_map_bind ok_type_subst ; eauto ; try rewrite concat_assoc.
+              apply_empty ok_type_weakening. apply* ok_pat_ok_type. constructors...
+              constructors... apply ok_pat_bsubst. apply* ok_pat_strengthening.
+          - replaces (BindMatch ([x => t2]t) p false) with (bsubst x t2 (BindMatch t p false))...
+            apply_ih_map_bind H3 ; auto. constructors...
+            apply ok_pat_bsubst. apply* ok_pat_strengthening. }
+        { Case "TmNever". constructor... apply* contradictory_subst. }
+        { Case "TmType". apply_fresh TType as T... rewrite* Topen_t_subst_comm.
+          replaces BindTName with (bsubst x t2 BindTName)...
+          apply_ih_map_bind H0 ; auto. constructor... }
+        { Case "TmConDef". apply_fresh TConDef as K...
+          - replaces (BindTVar (KiData d)) with (bsubst x t2 (BindTVar (KiData d)))...
+            apply_ih_map_bind ok_type_subst ; auto. rewrite~ concat_assoc. constructor...
+          - binds_cases H1 ; auto.
+            replaces BindTName with (bsubst x t2 BindTName)...
+          - replaces (BindCon d ty1 (FTName T))
+              with (bsubst x t2 (BindCon d ty1 (FTName T)))...
+            rewrite* Kopen_t_subst_comm. apply_ih_map_bind H3 ; auto.
+            apply_fresh EnvCon as X...
+            { replaces (BindTVar (KiData d)) with (bsubst x t2 (BindTVar (KiData d)))...
+              apply_ih_map_bind ok_type_subst ; auto. rewrite~ concat_assoc. constructor... }
+            { binds_cases H1 ; auto.
+              replaces BindTName with (bsubst x t2 BindTName)... } }
+        { Case "TmSem". apply_fresh TSem as y...
+          - apply ok_pat_bsubst. apply* ok_pat_strengthening.
+          - replaces (BindVar ty1') with (bsubst x t2 (BindVar ty1'))...
+            rewrite subst_open_comm... apply_ih_map_bind H2 ; auto.
+            constructor... applys ok_type_subst... applys* ok_pat_ok_type. }
+        { Case "TmSemApp". constructors...
+          apply exhaustive_bsubst. apply* exhaustive_strengthening. }
       Qed.
 
       Lemma ok_type_notin :
@@ -596,88 +1051,118 @@ Module TypingProps (P : PAT).
           apply binds_get in H0.
           fequals. }
         { Case "TyAll". pick_fresh Y.
-          forwards~ Htk: H1 Y.
-          forwards~ Hnin1 : topen_notin Htk. }
+          forwards~ Hnin : topen_notin (H1 Y). }
       Qed.
 
-      Lemma env_bsubst_fresh :
+      Lemma ok_term_notin :
+        forall Gamma t T X,
+          Gamma |= t ~: T ->
+          X # Gamma ->
+          X \notin tfv_t t.
+      Proof with eauto using ok_type_notin.
+        introv Htype Hfresh.
+        induction Htype; simpls...
+        - pick_fresh x. forwards Hnin : open_notin (H1 x)...
+        - pick_fresh Y. forwards~ Hnin : topen_t_notin (H1 Y).
+        - pick_fresh M. pick_fresh x. forwards~ Hnin1 : open_notin (H1 M x).
+          forwards~ Hnin2 : H3 M.
+        - pick_fresh T. forwards~ Hnin : Topen_t_notin (H0 T).
+        - pick_fresh K. forwards~ Hnin1 : Kopen_t_notin (H3 K).
+          forwards~ Hnin2 : ok_type_notin X (H0 K).
+          forwards~ Hnin2' : topen_notin Hnin2.
+        - pick_fresh x. forwards~ Hnin1 : open_notin (H2 x).
+          forwards~ Hnin2 : ok_type_notin X H.
+      Qed.
+
+      Lemma env_tbsubst_fresh :
         forall Gamma X T2,
           ok_env Gamma ->
           X # Gamma ->
-          Gamma = map (bsubst X T2) Gamma.
-      Proof with eauto using ok_env_push.
+          Gamma = map (tbsubst X T2) Gamma.
+      Proof.
         introv Henv Hfresh.
-        induction Gamma using env_ind.
-        { Case "Empty". rewrite~ map_empty. }
-        { Case "Push". autorewrite with rew_env_map.
-          rewrite <- IHGamma...
-          destruct~ v ; repeat fequals ; unfold bsubst ; rewrite* tsubst_fresh.
-          { SCase "BindCon".
-            apply ok_env_con_inv in Henv as (? & ? & ? & ? & Htk & ?).
-            pick_fresh X'. forwards~ Hnin : ok_type_notin X (Htk X').
-            applys~ topen_notin Hnin. }
-          { SCase "BindVar".
-            apply ok_env_var_inv in Henv.
-            apply* ok_type_notin. } }
+        induction Henv ; autorewrite with rew_env_map ; repeat fequals ; simpls~.
+        { Case "BindCon". rewrite* tsubst_fresh.
+          pick_fresh X'. forwards~ Hnin : ok_type_notin X (H1 X').
+          applys~ topen_notin Hnin. }
+        { Case "BindVar". rewrite* tsubst_fresh.
+          apply* ok_type_notin. }
+        { Case "BindMatch". rewrite* tsubst_t_fresh.
+          apply* ok_term_notin. }
       Qed.
 
       Lemma ok_term_tsubst :
         forall G2 G1 t k T1 T2 X,
           G1 & X ~ BindTVar k & G2 |= t ~: T1 ->
           G1 |= T2 ~:: k ->
-          G1 & map (bsubst X T2) G2 |= [{X => T2}]t ~: ({X => T2}T1).
-      Proof with eauto using ok_env_strengthening, bsubst_ok_env, ok_type_lct with mcore.
+          ok_env (G1 & map (tbsubst X T2) G2) ->
+          G1 & map (tbsubst X T2) G2 |= [{X => T2}]t ~: ({X => T2}T1).
+      Proof with eauto using ok_data_tvar_strengthening, ok_kind_tvar_strengthening,
+          ok_data_tbsubst, ok_kind_tbsubst, ok_type_tsubst, ok_type_lct with mcore.
         introv hasType Henv.
         remember (G1 & X ~ BindTVar k & G2) as G. gen G2.
         induction hasType; intros; simpls; substs...
         { Case "TmFVar". constructor...
-          replaces (BindVar ({X => T2} ty)) with (bsubst X T2 (BindVar ty))...
+          replaces (BindVar ({X => T2} ty)) with (tbsubst X T2 (BindVar ty))...
           binds_cases H0 ; auto.
           assert (X # G1) by (applys ok_push_inv ; applys* ok_concat_inv_l G2).
-          rewrite* (env_bsubst_fresh G1 X T2). }
-        { Case "TmLam". apply_fresh* TLam as x.
-          + applys ok_type_tsubst...
-          + replaces (BindVar ({X => T2}ty1)) with (bsubst X T2 (BindVar ty1))...
-            rewrite tsubst_t_open_comm. apply_ih_map_bind H1 ; auto. }
-        { Case "TmTyLam". apply_fresh* TTyLam.
-          + apply ok_kind_bsubst. apply* ok_kind_tvar_strengthening.
-          + replaces (BindTVar k0) with (bsubst X T2 (BindTVar k0))...
-            rewrite tsubst_topen_comm... rewrite topen_t_tsubst_comm...
-            apply_ih_map_bind H1 ; auto. }
-        { Case "TmTyApp".
-          rewrite tsubst_topen_distr... constructors*.
-          apply* ok_type_tsubst. }
+          rewrite* (env_tbsubst_fresh G1 X T2). }
+        { Case "TmLam". apply_fresh TLam as x...
+          replaces (BindVar ({X => T2}ty1)) with (tbsubst X T2 (BindVar ty1))...
+          rewrite tsubst_t_open_comm. apply_ih_map_bind H1 ; auto.
+          constructor... }
+        { Case "TmTyLam". apply_fresh TTyLam...
+          replaces (BindTVar k0) with (tbsubst X T2 (BindTVar k0))...
+          rewrite tsubst_topen_comm... rewrite topen_t_tsubst_comm...
+          apply_ih_map_bind H1 ; auto. constructor... }
+        { Case "TmTyApp". rewrite tsubst_topen_distr... }
         { Case "TmCon".
           apply TCon with (d := d) (ty1 := {X => T2}ty1) ; try apply* ok_type_tsubst.
-          - replaces (BindCon d ({X => T2} ty1) (FTName T)) with (bsubst X T2 (BindCon d ty1 (FTName T)))...
+          - replaces (BindCon d ({X => T2} ty1) (FTName T)) with (tbsubst X T2 (BindCon d ty1 (FTName T)))...
             binds_cases H ; auto.
             assert (X # G1) by (applys ok_push_inv ; applys* ok_concat_inv_l G2).
-            rewrite* (env_bsubst_fresh G1 X T2).
+            rewrite* (env_tbsubst_fresh G1 X T2).
           - rewrite <- tsubst_topen_distr... }
-        { Case "TmMatch". apply_fresh* TMatch as x.
-          + applys* ok_pat_tsubst.
-          + replaces (BindVar ({X => T2}ty1')) with (bsubst X T2 (BindVar ty1'))...
-            rewrite tsubst_t_open_comm. apply_ih_map_bind H1 ; auto. }
+        { Case "TmMatch". apply_fresh TMatch ; intros...
+          - applys* ok_pat_tsubst.
+          - replaces (BindVar ({X => T2}ty1')) with (tbsubst X T2 (BindVar ty1'))...
+            replaces (BindMatch ([{X => T2}]t) p true) with (tbsubst X T2 (BindMatch t p true))...
+            rewrite tsubst_t_open_comm.
+            do_rew_2 concat_assoc_map_push (applys H1 M) ; auto. rewrite_all~ concat_assoc.
+            constructor~.
+            + constructors... applys* ok_pat_tsubst.
+            + apply_ih_map_bind ok_type_tsubst ; eauto ; try rewrite concat_assoc.
+              apply_empty ok_type_weakening. apply* ok_pat_ok_type. constructors...
+              constructors... apply* ok_pat_tsubst.
+          - replaces (BindMatch ([{X => T2}]t) p false) with (tbsubst X T2 (BindMatch t p false))...
+            apply_ih_map_bind H3 ; auto. constructors... apply* ok_pat_tsubst. }
+        { Case "TmNever". constructors... applys contradictory_tsubst... }
         { Case "TmType". apply_fresh TType.
-          replaces BindTName with (bsubst X T2 BindTName)...
-          rewrite Topen_t_tsubst_comm... apply_ih_map_bind H0 ; auto. }
+          replaces BindTName with (tbsubst X T2 BindTName)...
+          rewrite Topen_t_tsubst_comm... apply_ih_map_bind H0 ; auto.
+          constructor... }
         { Case "TmConDef".
           apply_fresh TConDef.
-          - apply* ok_data_bsubst. apply* ok_data_tvar_strengthening.
-          - replaces (BindTVar (KiData d)) with (bsubst X T2 (BindTVar (KiData d)))...
+          - apply* ok_data_tbsubst. apply* ok_data_tvar_strengthening.
+          - replaces (BindTVar (KiData d)) with (tbsubst X T2 (BindTVar (KiData d)))...
             rewrite tsubst_topen_comm...
-            apply_ih_map_bind ok_type_tsubst ; eauto ; try rewrite* concat_assoc.
-            apply_ih_map_bind bsubst_ok_env ; eauto ; try rewrite* concat_assoc.
+            apply_ih_map_bind ok_type_tsubst ; eauto ; try rewrite* concat_assoc. constructor...
           - binds_cases H1 ; auto.
-            replaces BindTName with (bsubst X T2 BindTName) ; auto.
-          - replaces (BindCon d ({X => T2} ty1) (FTName T)) with (bsubst X T2 (BindCon d ty1 (FTName T)))...
-            rewrite Kopen_t_tsubst_comm... apply_ih_map_bind H3 ; auto. }
-        { Case "TmSem". apply_fresh* TSem as x.
-          + applys ok_type_tsubst...
+            replaces BindTName with (tbsubst X T2 BindTName) ; auto.
+          - replaces (BindCon d ({X => T2} ty1) (FTName T)) with (tbsubst X T2 (BindCon d ty1 (FTName T)))...
+            rewrite Kopen_t_tsubst_comm... apply_ih_map_bind H3 ; auto.
+            apply_fresh EnvCon...
+            + replaces (BindTVar (KiData d)) with (tbsubst X T2 (BindTVar (KiData d)))...
+              rewrite tsubst_topen_comm...
+              apply_ih_map_bind ok_type_tsubst ; eauto ; try rewrite* concat_assoc. constructor...
+            + binds_cases H1 ; auto.
+              replaces BindTName with (tbsubst X T2 BindTName) ; auto. }
+        { Case "TmSem". apply_fresh TSem as x...
           + applys* ok_pat_tsubst.
-          + replaces (BindVar ({X => T2}ty1')) with (bsubst X T2 (BindVar ty1'))...
-            rewrite tsubst_t_open_comm. apply_ih_map_bind H2 ; auto. }
-        { Case "TmSemApp". constructors*. apply* pats_exhaustive_tsubst. }
+          + replaces (BindVar ({X => T2}ty1')) with (tbsubst X T2 (BindVar ty1'))...
+            rewrite tsubst_t_open_comm. apply_ih_map_bind H2 ; auto.
+            constructor... applys* ok_type_tsubst. apply* ok_pat_ok_type. }
+        { Case "TmSemApp". constructors*. apply* exhaustive_tsubst. }
       Qed.
 
       Lemma ok_data_comm :
@@ -745,10 +1230,14 @@ Module TypingProps (P : PAT).
         { Case "TmCon". constructors... binds_cases H...
           apply* binds_concat_left_ok. apply* binds_concat_left_ok.
           applys* ok_concat_inv_l G2. }
-        { Case "TmMatch". apply_fresh TMatch as x...
+        { Case "TmMatch". apply_fresh TMatch ; intros...
           + apply* ok_pat_comm.
-          + apply_ih_bind H1 ; auto. constructor...
-            apply~ ok_type_comm. apply* ok_pat_ok_type. }
+          + do_rew_2 concat_assoc (applys H1 M) ; auto. easy.
+            constructor~. constructors... apply* ok_pat_comm.
+            apply_empty~ ok_type_weakening. apply~ ok_type_comm. apply* ok_pat_ok_type.
+            constructors... apply* ok_pat_comm.
+          + apply_ih_bind H3 ; eauto ; auto. constructors... apply* ok_pat_comm. }
+        { Case "TmNever". constructor... apply~ contradictory_comm. }
         { Case "TmType". apply_fresh TType as T...
           apply_ih_bind H0 ; auto. constructor... }
         { Case "TmConDef".
@@ -763,180 +1252,7 @@ Module TypingProps (P : PAT).
         { Case "TmSem". apply_fresh TSem as x...
           + apply* ok_pat_comm.
           + apply_ih_bind H2 ; auto. constructor... apply~ ok_type_comm. apply* ok_pat_ok_type. }
-        { Case "TmSemApp". constructors~. apply~ pats_exhaustive_comm. }
-      Qed.
-
-      Lemma ok_env_binds_con_inv :
-        forall Gamma K d ty T,
-          ok_env Gamma  ->
-          binds K (BindCon d ty T) Gamma ->
-          exists L T',
-            T = FTName T'
-            /\ ok_data Gamma d
-            /\ (forall X, X \notin L -> Gamma & X ~ BindTVar (KiData d) |= {0 ~> TyFVar X}ty ~:: KiType)
-            /\ binds T' BindTName Gamma.
-      Proof.
-        introv Henv Hbinds.
-        induction Gamma using env_ind.
-        - false. apply* binds_empty_inv.
-        - binds_cases Hbinds.
-          + destruct~ IHGamma as (L & T' & Heq & Hd & Htk & Hbinds'). apply* ok_env_push.
-            exists (L \u dom Gamma \u \{x}) T'. splits*. apply_empty~ ok_data_weakening.
-            introv Hfresh. apply~ ok_type_weakening. constructor~. constructor.
-            apply_empty~ ok_data_weakening. apply* binds_concat_left_ok.
-          + inverts EQ. forwards* (L & T' & Heq & Hd & Htk & Hbinds') : ok_env_con_inv.
-            exists (L \u dom Gamma \u \{K}) T'. splits~. apply_empty~ ok_data_weakening.
-            introv Hfresh. apply~ ok_type_weakening. constructor~. constructor.
-            apply_empty~ ok_data_weakening. apply* binds_concat_left_ok.
-      Qed.
-
-      Lemma ok_env_binds_tvar_inv :
-        forall Gamma X k,
-          ok_env Gamma ->
-          binds X (BindTVar k) Gamma ->
-          ok_kind Gamma k.
-      Proof.
-        introv Henv Hbinds.
-        induction Gamma using env_ind.
-        - false. apply* binds_empty_inv.
-        - binds_cases Hbinds.
-          + apply_empty~ ok_kind_weakening. apply~ IHGamma. apply* ok_env_push.
-          + substs. forwards* Hk: ok_env_tvar_inv. apply_empty~ ok_kind_weakening.
-      Qed.
-
-      Lemma ok_env_binds_var_inv :
-        forall Gamma x ty,
-          ok_env Gamma ->
-          binds x (BindVar ty) Gamma ->
-          Gamma |= ty ~:: KiType.
-      Proof.
-        introv Henv Hbinds.
-        induction Gamma using env_ind.
-          - false. apply* binds_empty_inv.
-          - binds_cases Hbinds.
-            + apply_empty~ ok_type_weakening. forwards~ ?: ok_env_push Henv.
-            + inverts EQ. apply_empty~ ok_type_weakening. apply* ok_env_var_inv.
-      Qed.
-
-      Lemma ok_type_ok_kind :
-        forall Gamma T k,
-          Gamma |= T ~:: k ->
-          ok_kind Gamma k.
-      Proof. introv Htk. induction* Htk. apply* ok_env_binds_tvar_inv. Qed.
-
-      Lemma ok_data_notin_T :
-        forall Gamma d X,
-          ok_data Gamma d ->
-          X # Gamma ->
-          X \notin Tfv_d d.
-      Proof.
-        introv Hd Hfresh. unfolds Tfv_d.
-        induction Hd ; rew_listx ; simpls~.
-        rewrite notin_union. splits*.
-        - rewrite notin_singleton. intro. substs.
-          forwards~ Hin : get_some_inv H0.
-      Qed.
-
-      Lemma ok_kind_notin_T :
-        forall Gamma k X,
-          ok_kind Gamma k ->
-          X # Gamma ->
-          X \notin Tfv_k k.
-      Proof.
-        introv Hk Hfresh. unfolds Tfv_k.
-        destruct~ Hk. apply* ok_data_notin_T.
-      Qed.
-
-      Lemma assoc_data_in :
-        forall d T Ks,
-          mem (FTName T, Ks) d -> T \in Tfv_d d.
-      Proof.
-        introv Hassoc. unfolds Tfv_d.
-        induction Hassoc ; rew_listx ; simpls~.
-        - rewrite~ in_union. rewrite~ in_singleton.
-        - destruct y. rewrite~ in_union.
-      Qed.
-
-      Lemma ok_type_notin_T :
-        forall Gamma T k X,
-          Gamma |= T ~:: k ->
-          X # Gamma ->
-          X \notin Tfv_ty T.
-      Proof with eauto using ok_data_notin_T, ok_kind_notin_T.
-        introv Htk Hfresh.
-        induction Htk; simpls...
-        { Case "TyAll". rewrite notin_union. splits...
-          pick_fresh Y. forwards~ Htk: H1 Y.
-          rewrite topen_notin_T in Htk ; simpls~. }
-        { Case "TyCon". rewrite notin_union. splits~.
-          forwards Hk: ok_type_ok_kind Htk.
-          forwards~ Hnin : ok_kind_notin_T X Hk.
-          assert (X <> T) by (intro ; substs ; apply Hnin ; applys* assoc_data_in).
-          auto. }
-      Qed.
-
-
-      Lemma ok_data_tname_strengthening :
-        forall G2 G1 T d,
-          T \notin Tfv_d d ->
-          ok_data (G1 & T ~ BindTName & G2) d ->
-          ok_data (G1 & G2) d.
-      Proof.
-        introv Hfv Hd. remember (G1 & T ~ BindTName & G2) as Gamma eqn:HGamma.
-        unfolds Tfv_d. induction Hd ; substs ; constructor ; rew_listx in Hfv ; simpls~.
-        - binds_cases H0 ; auto. notin_false.
-        - induction* Ks. inverts H1.
-          constructors~. binds_cases H8 ; eauto.
-      Qed.
-
-      Lemma ok_kind_tname_strengthening :
-        forall T G2 G1 k,
-          T \notin Tfv_k k ->
-          ok_kind (G1 & T ~ BindTName & G2) k ->
-          ok_kind (G1 & G2) k.
-      Proof with eauto using ok_data_tname_strengthening with mcore.
-        introv Hfv Hk.
-        remember (G1 & T ~ BindTName & G2) as Gamma eqn:HGamma.
-        induction Hk ; substs...
-      Qed.
-
-      Lemma data_sub_notin_T :
-        forall T d1 d2,
-          T \notin Tfv_d d1 ->
-          data_sub d2 d1 ->
-          T \notin Tfv_d d2.
-      Proof with eauto.
-        introv Hnin Hsub. unfolds data_sub. unfolds Tfv_d.
-        induction d2 ; rew_listx ; simpls~.
-        rewrite notin_union ; split~. destruct a. destruct~ t.
-        assert (T <> v)... intro ; substs.
-        forwards~ (?&Hmem&?) : Hsub. forwards~ (?&?&Heq) : mem_inv_middle Hmem.
-        substs. rew_listx* in Hnin. simpls.
-        notin_false.
-      Qed.
-
-      Lemma ok_type_tname_strengthening :
-        forall T G2 G1 ty k,
-          T \notin Tfv_ty ty ->
-          G1 & T ~ BindTName & G2 |= ty ~:: k ->
-          ok_env (G1 & G2) ->
-          G1 & G2 |= ty ~:: k.
-      Proof with eauto using ok_data_tname_strengthening, ok_kind_tname_strengthening with mcore.
-        introv Hfv Htk Henv.
-        remember (G1 & T ~ BindTName & G2) as Gamma eqn:HGamma. gen G2.
-        induction Htk ; intros ; simpls ; substs...
-        { Case "TyFVar". constructor~. binds_cases H0 ; auto. }
-        { Case "TyAll". rewrite notin_union in Hfv ; destruct Hfv.
-          apply_fresh KAll as X...
-          apply_ih_bind H1 ; auto. rewrite topen_notin_T ; simpls~. constructors... }
-        { Case "TySem". constructor~. apply* Forall_pred_incl.
-          intros p (ty1'&Hwf). eexists. apply* ok_pat_tname_strengthening ; auto. }
-        { Case "TyDataSub". applys~ KDataSub d1.
-          apply* ok_data_tname_strengthening.
-          forwards~ Hd1 : IHHtk. forwards Hk : ok_type_ok_kind Hd1.
-          inverts Hk. forwards~ Hnin : ok_data_notin_T T H3.
-          forwards* (Hfr1&Hfr2) : ok_middle_inv G1 G2.
-          apply* data_sub_notin_T. }
+        { Case "TmSemApp". constructors~. apply~ exhaustive_comm. }
       Qed.
 
       Lemma env_Tbsubst_fresh :
@@ -944,27 +1260,22 @@ Module TypingProps (P : PAT).
           ok_env Gamma ->
           X # Gamma ->
           Gamma = map (Tbsubst X T) Gamma.
-      Proof with eauto using ok_env_push.
+      Proof.
         introv Henv Hfresh.
-        induction Gamma using env_ind.
-        { Case "Empty". rewrite~ map_empty. }
-        { Case "Push". autorewrite with rew_env_map.
-          rewrite <- IHGamma...
-          destruct~ v ; repeat fequals ; unfold Tbsubst.
-          { SCase "BindCon".
-            apply ok_env_con_inv in Henv as (? & ? & ? & ? & Htk & ?). fequals.
-            - rewrite~ Tsubst_d_fresh. forwards~ Hnin : ok_data_notin_T X H0.
-            - rewrite~ Tsubst_ty_fresh. pick_fresh X'.
-              forwards~ Hnin : ok_type_notin_T X (Htk X').
-              rewrite topen_notin_T in Hnin ; simpls~.
-            - destruct t0 ; solve_var. inverts H. forwards* Hin : get_some_inv x1.
-              assert (Hnin: x1 # Gamma) by auto. contradiction. }
-          { SCase "BindTVar".
-            apply ok_env_tvar_inv in Henv. fequals.
-            rewrite~ Tsubst_k_fresh. apply* ok_kind_notin_T. }
-          { SCase "BindVar".
-            apply ok_env_var_inv in Henv. fequals.
-            rewrite~ Tsubst_ty_fresh. apply* ok_type_notin_T. } }
+        induction Henv ; autorewrite with rew_env_map ; repeat fequals ; simpls~.
+        { Case "BindCon". fequals.
+          - rewrite~ Tsubst_d_fresh. forwards~ Hnin : ok_data_notin_T X H0.
+          - rewrite~ Tsubst_ty_fresh. pick_fresh X'.
+            forwards~ Hnin : ok_type_notin_T X (H1 X').
+            rewrite topen_notin_T in Hnin ; simpls~.
+          - solve_var. forwards* Hin : get_some_inv T0.
+            assert (Hnin: T0 # Gamma) by auto. contradiction. }
+        { Case "BindTVar". fequals.
+          rewrite~ Tsubst_k_fresh. apply* ok_kind_notin_T. }
+        { Case "BindVar". fequals.
+          rewrite~ Tsubst_ty_fresh. apply* ok_type_notin_T. }
+        { Case "BindMatch". fequals.
+          rewrite~ Tsubst_t_fresh. apply* ok_term_notin_T. }
       Qed.
 
       Lemma assoc_Tsubst :
@@ -1056,7 +1367,7 @@ Module TypingProps (P : PAT).
           G1 & T' ~ BindTName &
             map (Tbsubst T (FTName T')) G2 |=
                 Tsubst_ty T (FTName T') ty ~:: Tsubst_k T (FTName T') k.
-      Proof with eauto with mcore.
+      Proof with eauto using ok_kind_Tsubst, ok_data_Tsubst with mcore.
         introv Htk Hfresh Henv. assert (Henv' : ok_env G1)
           by (applys ok_env_concat ; applys* ok_env_concat).
         remember (G1 & T ~ BindTName & G2) as G. gen G2.
@@ -1067,68 +1378,30 @@ Module TypingProps (P : PAT).
           apply~ binds_concat_left. apply* binds_concat_left_ok.
           assert (T # G1) by (applys ok_push_inv ; applys* ok_concat_inv_l G2).
           rewrite~ (env_Tbsubst_fresh G1 T (FTName T')). }
-        { Case "TyAll". apply_fresh KAll as X.
-          + apply ok_kind_Tsubst...
-          + replaces (BindTVar (Tsubst_k T (FTName T') k))
-              with (Tbsubst T (FTName T') (BindTVar k))...
-            rewrite <- Tsubst_ty_topen_comm. apply_ih_map_bind H1 ; auto.
-            constructor~. apply~ ok_kind_Tsubst... }
+        { Case "TyAll". apply_fresh KAll as X...
+          replaces (BindTVar (Tsubst_k T (FTName T') k))
+            with (Tbsubst T (FTName T') (BindTVar k))...
+          rewrite <- Tsubst_ty_topen_comm. apply_ih_map_bind H1 ; auto.
+          constructor... }
         { Case "TyCon".
           asserts (S, Heq): (lcT (Tsubst T (FTName T') (FTName T0))). solve_var.
           simpls. rewrite Heq. apply KCon with (d := Tsubst_d T (FTName T') d) (Ks := Ks)...
           rewrite <- Heq. applys~ assoc_Tsubst. }
         { Case "TySem". constructor~. apply* Forall_pred_incl.
           intros p (ty1'&Hwf). eexists. apply ok_pat_Tsubst ; eauto. apply* ok_type_ok_env. }
-        { Case "TyData". constructor~. apply~ ok_data_Tsubst... }
-        { Case "TyDataSub". applys~ KDataSub (Tsubst_d T (FTName T') d1).
-          - apply~ data_sub_Tsubst.
-          - apply~ ok_data_Tsubst. apply* ok_type_ok_env. }
-      Qed.
-
-      Lemma Tbsubst_ok_env :
-        forall G1 G2 T T',
-          ok_env (G1 & T ~ BindTName & G2) ->
-          T' # G1 & T ~ BindTName & G2 ->
-          ok_env (G1 & T' ~ BindTName & map (Tbsubst T (FTName T')) G2).
-      Proof with eauto using ok_data_Tsubst, ok_kind_Tsubst, ok_type_Tsubst with mcore.
-        introv Henv Hfresh. assert (Henv1 : ok_env G1)
-          by (applys ok_env_concat; applys* ok_env_concat).
-        induction G2 using env_ind.
-        { Case "Empty". autorewrite with rew_env_map rew_env_concat in *.
-          constructor~. }
-        { Case "Push". autorewrite with rew_env_map rew_env_concat in *.
-          specializes IHG2 (ok_env_push _ _ _ Henv).
-          lets [? Hdisj] : ok_push_inv (ok_env_ok _ Henv).
-          assert (ok_env (G1 & T ~ BindTName & G2)) by apply* ok_env_concat.
-          destruct v.
-          { SCase "BindTName". constructor~. }
-          { SCase "BindCon". forwards (L & T0 & Heq & Hd & Htk' & HT): ok_env_con_inv Henv.
-            substs. asserts (S, Heq): (lcT (Tsubst T (FTName T') (FTName T0))). solve_var.
-            simpls. rewrite Heq. apply_fresh EnvCon as X...
-            - replaces (BindTVar (KiData (Tsubst_d T (FTName T') d)))
-                with (Tbsubst T (FTName T') (BindTVar (KiData d))) ; auto.
-              replaces KiType with (Tsubst_k T (FTName T') KiType) ; auto.
-              rewrite <- Tsubst_ty_topen_comm.
-              apply_ih_map_bind ok_type_Tsubst ; try rewrite* concat_assoc ; auto.
-              constructor...
-            - solve_var ; inverts~ Heq. binds_cases HT ; auto.
-              apply~ binds_concat_left. apply* binds_concat_left_ok.
-              replaces BindTName with (Tbsubst T (FTName T') BindTName) ; eauto. }
-          { SCase "BindTVar". forwards Hk: ok_env_tvar_inv Henv. constructor... }
-          { SCase "BindVar". forwards Htk': ok_env_var_inv Henv. constructor~.
-            replaces KiType with (Tsubst_k T (FTName T') KiType)... }
-          (* { SCase "BindMatch". constructor~. } *)
-        }
+        { Case "TyDataSub". applys KDataSub (Tsubst_d T (FTName T') d1)...
+          apply~ data_sub_Tsubst. }
       Qed.
 
       Lemma ok_term_Tsubst :
         forall G2 G1 T T' t ty,
           G1 & T ~ BindTName & G2 |= t ~: ty ->
           T' # G1 & T ~ BindTName & G2 ->
+          ok_env (G1 & T' ~ BindTName & map (Tbsubst T (FTName T')) G2) ->
           G1 & T' ~ BindTName &
             map (Tbsubst T (FTName T')) G2 |=
                 Tsubst_t T (FTName T') t ~: Tsubst_ty T (FTName T') ty.
-      Proof with eauto using Tbsubst_ok_env with mcore.
+      Proof with eauto using ok_type_Tsubst, ok_kind_Tsubst, ok_data_Tsubst with mcore.
         introv Htype. assert (Henv : ok_env G1)
           by (applys ok_env_concat ; applys* ok_env_concat).
         remember (G1 & T ~ BindTName & G2) as Gamma eqn:HGamma. gen G2.
@@ -1141,19 +1414,17 @@ Module TypingProps (P : PAT).
           rewrite~ (env_Tbsubst_fresh G1 T (FTName T')). }
         { Case "TmLam". apply_fresh TLam as x.
           + replaces KiType with (Tsubst_k T (FTName T') KiType)...
-            apply ok_type_Tsubst...
           + rewrite <- Tsubst_t_open_comm. folds (Tsubst_ty T (FTName T') ty1).
             replaces (BindVar (Tsubst_ty T (FTName T') ty1))
               with (Tbsubst T (FTName T') (BindVar ty1))...
-            apply_ih_map_bind H1 ; auto. }
-        { Case "TmTyLam". apply_fresh TTyLam as X.
-          + apply ok_kind_Tsubst...
-          + rewrite <- Tsubst_t_topen_comm. rewrite <- Tsubst_ty_topen_comm.
-            replaces (BindTVar (Tsubst_k T (FTName T') k))
-              with (Tbsubst T (FTName T') (BindTVar k))...
-            apply_ih_map_bind H1 ; auto. }
-        { Case "TmTyApp". rewrite Tsubst_ty_topen_distr. constructors*.
-          apply ok_type_Tsubst... }
+            apply_ih_map_bind H1 ; auto. constructor...
+            replaces KiType with (Tsubst_k T (FTName T') KiType)... }
+        { Case "TmTyLam". apply_fresh TTyLam as X...
+          rewrite <- Tsubst_t_topen_comm. rewrite <- Tsubst_ty_topen_comm.
+          replaces (BindTVar (Tsubst_k T (FTName T') k))
+            with (Tbsubst T (FTName T') (BindTVar k))...
+          apply_ih_map_bind H1 ; auto. constructor... }
+        { Case "TmTyApp". rewrite Tsubst_ty_topen_distr... }
         { Case "TmCon".
           asserts (S, Heq): (lcT (Tsubst T (FTName T') (FTName T0))). solve_var.
           simpls. rewrite Heq.
@@ -1165,46 +1436,71 @@ Module TypingProps (P : PAT).
             assert (T # G1) by (applys ok_push_inv ; applys* ok_concat_inv_l G2).
             rewrite~ (env_Tbsubst_fresh G1 T (FTName T')).
           - replaces (KiData (Tsubst_d T (FTName T') d)) with (Tsubst_k T (FTName T') (KiData d))...
-            apply* ok_type_Tsubst.
           - replaces (KiData [(FTName S, FCon K :: [])])
-              with (Tsubst_k T (FTName T') (KiData [(FTName T0, FCon K :: [])])). rewrite~ <- Heq.
-            apply* ok_type_Tsubst.
+              with (Tsubst_k T (FTName T') (KiData [(FTName T0, FCon K :: [])]))... rewrite~ <- Heq.
           - rewrite <- Tsubst_ty_topen_distr... }
-        { Case "TmMatch". apply_fresh TMatch as x...
-          + apply ok_pat_Tsubst...
-          + rewrite <- Tsubst_t_open_comm.
+        { Case "TmMatch". apply_fresh TMatch ; intros...
+          - apply ok_pat_Tsubst...
+          - rewrite <- Tsubst_t_open_comm. folds (Tsubst_t T (FTName T') t).
+            replaces (BindMatch (Tsubst_t T (FTName T') t) p true)
+              with (Tbsubst T (FTName T') (BindMatch t p true))...
             replaces (BindVar (Tsubst_ty T (FTName T') ty1'))
               with (Tbsubst T (FTName T') (BindVar ty1'))...
-            apply_ih_map_bind H1 ; auto. }
+            do_rew_2 concat_assoc_map_push (applys H1 M x) ; auto. rewrite_all~ concat_assoc.
+            constructor~.
+            + constructors... applys* ok_pat_Tsubst.
+            + replaces KiType with (Tsubst_k T (FTName T') KiType)...
+              apply_ih_map_bind ok_type_Tsubst ; eauto ; try rewrite concat_assoc.
+              apply_empty ok_type_weakening. apply* ok_pat_ok_type. constructors...
+              constructors... apply* ok_pat_Tsubst.
+          - folds (Tsubst_t T (FTName T') t).
+            replaces (BindMatch (Tsubst_t T (FTName T') t) p false)
+              with (Tbsubst T (FTName T') (BindMatch t p false))...
+            apply_ih_map_bind H3 ; auto. constructors... apply* ok_pat_Tsubst. }
+        { Case "TmNever". constructor.
+          - replaces KiType with (Tsubst_k T (FTName T') KiType)...
+          - apply contradictory_Tsubst... }
         { Case "TmType". apply_fresh TType as T0.
           replaces BindTName with (Tbsubst T (FTName T') BindTName)...
-          rewrite~ Tsubst_t_Topen_comm. apply_ih_map_bind H0 ; auto. }
+          rewrite~ Tsubst_t_Topen_comm. apply_ih_map_bind H0 ; auto. constructor... }
         { Case "TmConDef".
           asserts (S, Heq): (lcT (Tsubst T (FTName T') (FTName T0))). solve_var.
-          simpls. rewrite Heq. apply_fresh TConDef as X.
-          - apply ok_data_Tsubst...
+          simpls. rewrite Heq. apply_fresh TConDef as X...
           - replaces KiType with (Tsubst_k T (FTName T') KiType)...
             replaces (BindTVar (KiData (Tsubst_d T (FTName T') d)))
               with (Tbsubst T (FTName T') (BindTVar (KiData d)))...
             rewrite <- Tsubst_ty_topen_comm.
             apply_ih_map_bind ok_type_Tsubst ; eauto ; try rewrite* concat_assoc.
-            constructor... apply ok_kind_Tsubst...
+            constructor...
           - solve_var ; inverts~ Heq.
             binds_cases H1 ; auto.
             apply~ binds_concat_left. apply binds_concat_left_ok...
             replaces BindTName with (Tbsubst T (FTName T') BindTName)...
           - replaces (BindCon (Tsubst_d T (FTName T') d) (Tsubst_ty T (FTName T') ty1) (FTName S))
               with (Tbsubst T (FTName T') (BindCon d ty1 (FTName T0))). rewrite~ <- Heq.
-            rewrite Tsubst_t_Kopen_comm. apply_ih_map_bind H3 ; auto. }
+            rewrite Tsubst_t_Kopen_comm. apply_ih_map_bind H3 ; auto.
+            asserts (S0, Heq'): (lcT (Tsubst T (FTName T') (FTName T0))). solve_var.
+            simpls. rewrite Heq'. apply_fresh EnvCon ; intros...
+            + replaces KiType with (Tsubst_k T (FTName T') KiType)...
+              replaces (BindTVar (KiData (Tsubst_d T (FTName T') d)))
+                with (Tbsubst T (FTName T') (BindTVar (KiData d)))...
+              rewrite <- Tsubst_ty_topen_comm.
+              apply_ih_map_bind ok_type_Tsubst ; eauto ; try rewrite* concat_assoc.
+              constructor...
+            + solve_var ; inverts~ Heq'.
+              binds_cases H1 ; auto.
+              apply~ binds_concat_left. apply binds_concat_left_ok...
+              replaces BindTName with (Tbsubst T (FTName T') BindTName)... }
         { Case "TmSem". apply_fresh TSem as x.
           + replaces KiType with (Tsubst_k T (FTName T') KiType)...
-            apply ok_type_Tsubst...
           + apply ok_pat_Tsubst...
           + rewrite <- Tsubst_t_open_comm.
             replaces (BindVar (Tsubst_ty T (FTName T') ty1'))
               with (Tbsubst T (FTName T') (BindVar ty1'))...
-            apply_ih_map_bind H2 ; auto. }
-        { Case "TmSemApp". constructors*. apply* pats_exhaustive_Tsubst. }
+            apply_ih_map_bind H2 ; auto. constructor...
+            replaces KiType with (Tsubst_k T (FTName T') KiType)...
+            apply~ ok_type_Tsubst. applys ok_pat_ok_type H0. apply* ok_type_ok_env. }
+        { Case "TmSemApp". constructors*. apply* exhaustive_Tsubst. }
       Qed.
 
       Lemma ok_term_Topen_change :
@@ -1218,168 +1514,30 @@ Module TypingProps (P : PAT).
         rewrite~ (Tsubst_t_intro T (FTName T')).
         rewrite~ <- (Tsubst_ty_fresh T (FTName T')).
         apply_empty~ ok_term_Tsubst.
+        constructor~. applys* ok_env_concat.
       Qed.
 
-
-      Lemma ok_data_notin_K :
-        forall Gamma d X,
-          ok_data Gamma d ->
-          X # Gamma ->
-          X \notin Kfv_d d.
-      Proof.
-        introv Hd Hfresh. unfolds Kfv_d.
-        induction Hd ; rew_listx ; simpls~.
-        rewrite notin_union. splits*.
-        induction H1 ; rew_listx ; simpls~ ; rewrite notin_union ; splits~.
-        - rewrite notin_singleton. intro. substs.
-          forwards~ Hin : get_some_inv H3.
-      Qed.
-
-      Lemma ok_kind_notin_K :
-        forall Gamma k X,
-          ok_kind Gamma k ->
-          X # Gamma ->
-          X \notin Kfv_k k.
-      Proof.
-        introv Hk Hfresh. unfolds Kfv_k.
-        destruct~ Hk. apply* ok_data_notin_K.
-      Qed.
-
-      Lemma ok_type_notin_K :
-        forall Gamma T k X,
-          Gamma |= T ~:: k ->
-          X # Gamma ->
-          X \notin Kfv_ty T.
-      Proof with eauto using ok_data_notin_K, ok_kind_notin_K, ok_pat_notin_K.
-        introv Htk Hfresh.
-        induction Htk; simpls...
-        { Case "TyAll". rewrite notin_union. splits...
-          pick_fresh Y. forwards~ Htk: H1 Y.
-          rewrite topen_notin_K in Htk ; simpls~. }
-        { Case "TySem". rewrite_all notin_union. repeat split~.
-          induction ps ; rew_listx ; simpls~. rew_listx in H. destruct H as ((ty1'&Hfw)&?).
-          rewrite notin_union... }
-      Qed.
-
-      Lemma ok_data_con_strengthening :
-        forall K G2 G1 d' ty' T d,
-          K \notin Kfv_d d ->
-          ok_data (G1 & K ~ BindCon d' ty' T & G2) d ->
-          ok_data (G1 & G2) d.
-      Proof.
-        introv Hfv Hd. remember (G1 & K ~ BindCon d' ty' T & G2) as Gamma eqn:HGamma.
-        unfolds Kfv_d. induction Hd ; substs ; constructor ; rew_listx in Hfv ; simpls~.
-        - binds_cases H0 ; auto.
-        - induction* Ks. inverts H1. rew_listx in Hfv ; simpls~.
-          constructors~. binds_cases H8 ; eauto. notin_false.
-      Qed.
-
-      Lemma ok_kind_con_strengthening :
-        forall K G2 G1 d ty' T k,
-          K \notin Kfv_k k ->
-          ok_kind (G1 & K ~ BindCon d ty' T & G2) k ->
-          ok_kind (G1 & G2) k.
-      Proof with eauto using ok_data_con_strengthening with mcore.
-        introv Hfv Hk.
-        remember (G1 & K ~ BindCon d ty' T & G2) as Gamma eqn:HGamma.
-        induction Hk ; substs...
-      Qed.
-
-      Lemma data_sub_notin_K :
-        forall K d1 d2,
-          K \notin Kfv_d d1 ->
-          data_sub d2 d1 ->
-          K \notin Kfv_d d2.
-      Proof with eauto.
-        introv Hnin Hsub. unfolds data_sub. unfolds Kfv_d.
-        induction d2 ; rew_listx ; simpls~.
-        rewrite notin_union ; split~. destruct a.
-        forwards* (Ks'&Hmem&HsubK) : Hsub.
-        forwards~ (?&?&Heq) : mem_inv_middle Hmem. substs.
-        rew_listx* in Hnin ; simpls.
-        assert (HninK : K \notin fold varsM (fun K => Kfv K) Ks')...
-        clears IHd2 Hsub Hnin Hmem.
-        induction l ; rew_listx ; simpls~.
-        rewrite notin_union ; split~. destruct~ a.
-        assert (K <> v)... intro ; substs.
-        forwards~ Hmem : HsubK.
-        forwards~ (?&?&Heq) : mem_inv_middle Hmem. substs.
-        rew_listx* in HninK. simpls. notin_false.
-      Qed.
-
-      Lemma ok_type_con_strengthening :
-        forall K G2 G1 d ty' T ty k,
-          K \notin Kfv_ty ty ->
-          G1 & K ~ BindCon d ty' T & G2 |= ty ~:: k ->
-          ok_env (G1 & G2) ->
-          G1 & G2 |= ty ~:: k.
-      Proof with eauto using ok_data_con_strengthening, ok_kind_con_strengthening with mcore.
-        introv Hfv Htk Henv.
-        remember (G1 & K ~ BindCon d ty' T & G2) as Gamma eqn:HGamma. gen G2.
-        induction Htk ; intros ; simpls ; substs...
-        { Case "TyFVar". constructor~. binds_cases H0 ; auto. }
-        { Case "TyAll". rewrite notin_union in Hfv ; destruct Hfv.
-          apply_fresh KAll as X...
-          apply_ih_bind H1 ; auto. rewrite topen_notin_K ; simpls~. constructors... }
-        { Case "TySem". constructor~. apply* Forall_pred_incl.
-          intros p (ty1'&Hwf). eexists. apply* ok_pat_con_strengthening ; auto. }
-        { Case "TyDataSub". applys~ KDataSub d1.
-          apply* ok_data_con_strengthening.
-          forwards~ Hd1 : IHHtk. forwards Hk : ok_type_ok_kind Hd1.
-          inverts Hk. forwards~ Hnin : ok_data_notin_K K H3.
-          forwards* (Hfr1&Hfr2) : ok_middle_inv G1 G2.
-          apply* data_sub_notin_K. }
-      Qed.
-
-      Lemma ok_term_ok_type :
-        forall Gamma t ty,
-          Gamma |= t ~: ty ->
-          Gamma |= ty ~:: KiType.
-      Proof with eauto with mcore.
-        introv Htype.
-        induction* Htype.
-        - apply* ok_env_binds_var_inv.
-        - constructor~. pick_fresh x. forwards~ Htk : H1 x.
-          apply_empty* ok_type_strengthening.
-        - inverts~ IHHtype1.
-        - inverts IHHtype. pick_fresh X. rewrite~ (tsubst_intro X).
-          apply_empty* ok_type_tsubst.
-        - inverts~ IHHtype.
-        - inverts~ IHHtype.
-        - inverts~ IHHtype.
-        - pick_fresh T. apply_empty* (ok_type_tname_strengthening T).
-        - pick_fresh K. apply_empty* (ok_type_con_strengthening K).
-        - constructor ; rew_listx*.
-          pick_fresh x. forwards~ Htk : H2 x.
-          apply_empty* ok_type_strengthening.
-        - inverts IHHtype1. inverts IHHtype2. constructor ; rew_listx~.
-        - inverts~ IHHtype1.
-      Qed.
 
       Lemma env_Kbsubst_fresh :
         forall Gamma X K,
           ok_env Gamma ->
           X # Gamma ->
           Gamma = map (Kbsubst X K) Gamma.
-      Proof with eauto using ok_env_push.
+      Proof.
         introv Henv Hfresh.
-        induction Gamma using env_ind.
-        { Case "Empty". rewrite~ map_empty. }
-        { Case "Push". autorewrite with rew_env_map.
-          rewrite <- IHGamma...
-          destruct~ v ; repeat fequals ; unfold Kbsubst.
-          { SCase "BindCon".
-            apply ok_env_con_inv in Henv as (? & ? & ? & ? & Htk & ?). fequals.
-            - rewrite~ Ksubst_d_fresh. forwards~ Hnin : ok_data_notin_K X H0.
-            - rewrite~ Ksubst_ty_fresh. pick_fresh X'.
-              forwards~ Hnin : ok_type_notin_K X (Htk X').
-              rewrite topen_notin_K in Hnin ; simpls~. }
-          { SCase "BindTVar".
-            apply ok_env_tvar_inv in Henv. fequals.
-            rewrite~ Ksubst_k_fresh. apply* ok_kind_notin_K. }
-          { SCase "BindVar".
-            apply ok_env_var_inv in Henv. fequals.
-            rewrite~ Ksubst_ty_fresh. apply* ok_type_notin_K. } }
+        induction Henv ; autorewrite with rew_env_map ; repeat fequals ; simpls~.
+        { Case "BindCon". fequals.
+          - rewrite~ Ksubst_d_fresh. forwards~ Hnin : ok_data_notin_K X H0.
+          - rewrite~ Ksubst_ty_fresh. pick_fresh X'.
+            forwards~ Hnin : ok_type_notin_K X (H1 X').
+            rewrite topen_notin_K in Hnin ; simpls~. }
+        { Case "BindTVar". fequals.
+          rewrite~ Ksubst_k_fresh. apply* ok_kind_notin_K. }
+        { Case "BindVar". fequals.
+          rewrite~ Ksubst_ty_fresh. apply* ok_type_notin_K. }
+        { Case "BindMatch". fequals.
+          - rewrite~ Ksubst_t_fresh. apply* ok_term_notin_K.
+          - rewrite~ Ksubst_p_fresh. apply* ok_pat_notin_K. }
       Qed.
 
       Lemma assoc_Ksubst :
@@ -1495,7 +1653,7 @@ Module TypingProps (P : PAT).
           G1 & K' ~ BindCon d ty' T &
             map (Kbsubst K (FCon K')) G2 |=
                 Ksubst_ty K (FCon K') ty ~:: Ksubst_k K (FCon K') k.
-      Proof with eauto with mcore.
+      Proof with eauto using ok_kind_Ksubst, ok_data_Ksubst with mcore.
         introv Htk Hfresh Henv. assert (Henv' : ok_env G1)
           by (applys ok_env_concat ; applys* ok_env_concat).
         remember (G1 & K ~ BindCon d ty' T & G2). gen G2.
@@ -1506,68 +1664,30 @@ Module TypingProps (P : PAT).
           apply~ binds_concat_left. apply* binds_concat_left_ok.
           assert (K # G1) by (applys ok_push_inv ; applys* ok_concat_inv_l G2).
           rewrite~ (env_Kbsubst_fresh G1 K (FCon K')). }
-        { Case "TyAll". apply_fresh KAll as X.
-          + apply ok_kind_Ksubst...
-          + replaces (BindTVar (Ksubst_k K (FCon K') k))
-              with (Kbsubst K (FCon K') (BindTVar k))...
-            rewrite <- Ksubst_ty_topen_comm. apply_ih_map_bind H1 ; auto.
-            constructor... apply ok_kind_Ksubst... }
+        { Case "TyAll". apply_fresh KAll as X...
+          replaces (BindTVar (Ksubst_k K (FCon K') k))
+            with (Kbsubst K (FCon K') (BindTVar k))...
+          rewrite <- Ksubst_ty_topen_comm. apply_ih_map_bind H1 ; auto.
+          constructor... }
         { Case "TyCon".
           apply KCon with (d := Ksubst_d K (FCon K') d0) (Ks := LibList.map (Ksubst K (FCon K')) Ks)...
           apply~ assoc_Ksubst. }
         { Case "TySem". constructor~. rewrite~ Forall_map_eq.
           apply* Forall_pred_incl. intros p (ty1'&Hwf). eexists.
           apply ok_pat_Ksubst ; eauto. apply* ok_type_ok_env. }
-        { Case "TyData". constructor~. apply~ ok_data_Ksubst. }
-        { Case "TyDataSub". applys~ KDataSub (Ksubst_d K (FCon K') d1).
-          - apply~ data_sub_Ksubst.
-          - apply~ ok_data_Ksubst. apply* ok_type_ok_env. }
-      Qed.
-
-      Lemma Kbsubst_ok_env :
-        forall G1 G2 K K' d ty T,
-          ok_env (G1 & K ~ BindCon d ty T & G2) ->
-          K' # G1 & K ~ BindCon d ty T & G2 ->
-          ok_env (G1 & K' ~ BindCon d ty T & map (Kbsubst K (FCon K')) G2).
-      Proof with eauto using ok_data_Ksubst, ok_kind_Ksubst, ok_type_Ksubst with mcore.
-        introv Henv Hfresh. assert (Henv1 : ok_env G1)
-          by (applys ok_env_concat; applys* ok_env_concat).
-        forwards Henv': ok_env_concat Henv. forwards (?&?&?&?&?&?): ok_env_con_inv Henv'.
-        substs. induction G2 using env_ind.
-        { Case "Empty". autorewrite with rew_env_map rew_env_concat in *.
-          apply_fresh EnvCon... }
-        { Case "Push". autorewrite with rew_env_map rew_env_concat in *.
-          specializes IHG2 (ok_env_push _ _ _ Henv) ; auto.
-          lets [? Hdisj] : ok_push_inv (ok_env_ok _ Henv).
-          assert (ok_env (G1 & K ~ BindCon d ty (FTName x0) & G2)) by apply* ok_env_concat.
-          destruct v.
-          { SCase "BindTName". constructor~. }
-          { SCase "BindCon". forwards (L & T0 & Heq & Hd & Htk' & HT): ok_env_con_inv Henv.
-            substs. apply_fresh EnvCon as X...
-            - replaces (BindTVar (KiData (Ksubst_d K (FCon K') d0)))
-                with (Kbsubst K (FCon K') (BindTVar (KiData d0))) ; auto.
-              replaces KiType with (Ksubst_k K (FCon K') KiType) ; auto.
-              rewrite <- Ksubst_ty_topen_comm.
-              apply_ih_map_bind ok_type_Ksubst ; try rewrite* concat_assoc ; auto.
-              constructor...
-            - binds_cases HT ; auto.
-              apply~ binds_concat_left. apply* binds_concat_left_ok.
-              replaces BindTName with (Kbsubst K (FCon K') BindTName) ; eauto. }
-          { SCase "BindTVar". forwards Hk: ok_env_tvar_inv Henv. constructor... }
-          { SCase "BindVar". forwards Htk': ok_env_var_inv Henv. constructor~.
-            replaces KiType with (Ksubst_k K (FCon K') KiType)... }
-          (* { SCase "BindMatch". constructor~. } *)
-        }
+        { Case "TyDataSub". applys KDataSub (Ksubst_d K (FCon K') d1)...
+          apply~ data_sub_Ksubst. }
       Qed.
 
       Lemma ok_term_Ksubst :
         forall G2 G1 K K' d ty' T t ty,
           G1 & K ~ BindCon d ty' T & G2 |= t ~: ty ->
           K' # G1 & K ~ BindCon d ty' T & G2 ->
+          ok_env (G1 & K' ~ BindCon d ty' T & map (Kbsubst K (FCon K')) G2) ->
           G1 & K' ~ BindCon d ty' T &
             map (Kbsubst K (FCon K')) G2 |=
                 Ksubst_t K (FCon K') t ~: Ksubst_ty K (FCon K') ty.
-      Proof with eauto using Kbsubst_ok_env with mcore.
+      Proof with eauto using ok_type_Ksubst, ok_kind_Ksubst, ok_data_Ksubst with mcore.
         introv Htype. assert (Henv : ok_env G1)
           by (applys ok_env_concat ; applys* ok_env_concat).
         remember (G1 & K ~ BindCon d ty' T & G2). gen G2.
@@ -1580,19 +1700,17 @@ Module TypingProps (P : PAT).
           rewrite~ (env_Kbsubst_fresh G1 K (FCon K')). }
         { Case "TmLam". apply_fresh TLam as x.
           + replaces KiType with (Ksubst_k K (FCon K') KiType)...
-            apply ok_type_Ksubst...
           + rewrite <- Ksubst_t_open_comm. folds (Ksubst_ty K (FCon K') ty1).
             replaces (BindVar (Ksubst_ty K (FCon K') ty1))
               with (Kbsubst K (FCon K') (BindVar ty1))...
-            apply_ih_map_bind H1 ; auto. }
-        { Case "TmTyLam". apply_fresh TTyLam as X.
-          + apply ok_kind_Ksubst...
-          + rewrite <- Ksubst_t_topen_comm. rewrite <- Ksubst_ty_topen_comm.
-            replaces (BindTVar (Ksubst_k K (FCon K') k))
-              with (Kbsubst K (FCon K') (BindTVar k))...
-            apply_ih_map_bind H1 ; auto. }
-        { Case "TmTyApp". rewrite Ksubst_ty_topen_distr. constructors*.
-          apply ok_type_Ksubst... }
+            apply_ih_map_bind H1 ; auto. constructor...
+            replaces KiType with (Ksubst_k K (FCon K') KiType)... }
+        { Case "TmTyLam". apply_fresh TTyLam as X...
+          rewrite <- Ksubst_t_topen_comm. rewrite <- Ksubst_ty_topen_comm.
+          replaces (BindTVar (Ksubst_k K (FCon K') k))
+            with (Kbsubst K (FCon K') (BindTVar k))...
+          apply_ih_map_bind H1 ; auto. constructor... }
+        { Case "TmTyApp". rewrite Ksubst_ty_topen_distr... }
         { Case "TmCon".
           asserts (S, Heq): (lcK (Ksubst K (FCon K') (FCon K0))). solve_var.
           simpls. rewrite Heq.
@@ -1610,49 +1728,72 @@ Module TypingProps (P : PAT).
               apply~ binds_concat_left. apply* binds_concat_left_ok.
               rewrite~ (env_Kbsubst_fresh G1 K (FCon K')).
           - replaces (KiData (Ksubst_d K (FCon K') d0)) with (Ksubst_k K (FCon K') (KiData d0))...
-            apply* ok_type_Ksubst.
           - replaces (KiData [(FTName T0, FCon S :: [])])
-              with (Ksubst_k K (FCon K') (KiData [(FTName T0, FCon K0 :: [])])). rewrite~ <- Heq.
-            apply* ok_type_Ksubst.
+              with (Ksubst_k K (FCon K') (KiData [(FTName T0, FCon K0 :: [])]))... rewrite~ <- Heq.
           - rewrite <- Ksubst_ty_topen_distr... }
-        { Case "TmMatch". apply_fresh TMatch as x...
-          + apply ok_pat_Ksubst...
-          + rewrite <- Ksubst_t_open_comm.
+        { Case "TmMatch". apply_fresh TMatch ; intros...
+          - apply ok_pat_Ksubst...
+          - rewrite <- Ksubst_t_open_comm. folds (Ksubst_t K (FCon K') t).
+            replaces (BindMatch (Ksubst_t K (FCon K') t) (Ksubst_p K (FCon K') p) true)
+              with (Kbsubst K (FCon K') (BindMatch t p true))...
             replaces (BindVar (Ksubst_ty K (FCon K') ty1'))
               with (Kbsubst K (FCon K') (BindVar ty1'))...
-            apply_ih_map_bind H1 ; auto. }
+            do_rew_2 concat_assoc_map_push (applys H1 M x) ; auto. rewrite_all~ concat_assoc.
+            constructor~.
+            + constructors... applys* ok_pat_Ksubst.
+            + replaces KiType with (Ksubst_k K (FCon K') KiType)...
+              apply_ih_map_bind ok_type_Ksubst ; eauto ; try rewrite concat_assoc.
+              apply_empty ok_type_weakening. apply* ok_pat_ok_type. constructors...
+              constructors... apply* ok_pat_Ksubst.
+          - folds (Ksubst_t K (FCon K') t).
+            replaces (BindMatch (Ksubst_t K (FCon K') t) (Ksubst_p K (FCon K') p) false)
+              with (Kbsubst K (FCon K') (BindMatch t p false))...
+            apply_ih_map_bind H3 ; auto. constructors... apply* ok_pat_Ksubst. }
+        { Case "TmNever". constructor~.
+          - replaces KiType with (Ksubst_k K (FCon K') KiType)...
+          - apply contradictory_Ksubst... }
         { Case "TmType". apply_fresh TType as T0.
           replaces BindTName with (Kbsubst K (FCon K') BindTName)...
-          rewrite~ Ksubst_t_Topen_comm. apply_ih_map_bind H0 ; auto. }
-        { Case "TmConDef". apply_fresh TConDef as X.
-          - apply~ ok_data_Ksubst...
+          rewrite~ Ksubst_t_Topen_comm. apply_ih_map_bind H0 ; auto. constructor... }
+        { Case "TmConDef". apply_fresh TConDef as X...
           - replaces KiType with (Ksubst_k K (FCon K') KiType)...
             replaces (BindTVar (KiData (Ksubst_d K (FCon K') d0)))
               with (Kbsubst K (FCon K') (BindTVar (KiData d0)))...
             rewrite <- Ksubst_ty_topen_comm.
             apply_ih_map_bind ok_type_Ksubst ; eauto ; try rewrite* concat_assoc.
-            constructor... apply ok_kind_Ksubst...
+            constructor...
           - binds_cases H1 ; auto.
             apply~ binds_concat_left. apply binds_concat_left_ok...
             replaces BindTName with (Kbsubst K (FCon K') BindTName)...
           - replaces (BindCon (Ksubst_d K (FCon K') d0) (Ksubst_ty K (FCon K') ty1) (FTName T0))
               with (Kbsubst K (FCon K') (BindCon d0 ty1 (FTName T0)))...
-            rewrite~ Ksubst_t_Kopen_comm. apply_ih_map_bind H3 ; auto. }
+            rewrite~ Ksubst_t_Kopen_comm. apply_ih_map_bind H3 ; auto.
+            apply_fresh EnvCon as K...
+            + replaces KiType with (Ksubst_k K (FCon K') KiType)...
+              replaces (BindTVar (KiData (Ksubst_d K (FCon K') d0)))
+                with (Kbsubst K (FCon K') (BindTVar (KiData d0)))...
+              rewrite <- Ksubst_ty_topen_comm.
+              apply_ih_map_bind ok_type_Ksubst ; eauto ; try rewrite* concat_assoc.
+              constructor...
+            + binds_cases H1 ; auto.
+              apply~ binds_concat_left. apply binds_concat_left_ok...
+              replaces BindTName with (Kbsubst K (FCon K') BindTName)... }
         { Case "TmSem". apply_fresh TSem as x.
           + replaces KiType with (Ksubst_k K (FCon K') KiType)...
-            apply ok_type_Ksubst...
           + apply ok_pat_Ksubst...
           + rewrite <- Ksubst_t_open_comm.
             replaces (BindVar (Ksubst_ty K (FCon K') ty1'))
               with (Kbsubst K (FCon K') (BindVar ty1'))...
-            apply_ih_map_bind H2 ; auto. }
+            apply_ih_map_bind H2 ; auto. constructor~.
+            replaces KiType with (Ksubst_k K (FCon K') KiType)...
+            applys~ ok_type_Ksubst. apply* ok_pat_ok_type. }
         { Case "TmComp". simpls. rew_listx.
-          constructor... forwards* Hcomp: pats_compatible_Ksubst __ K'.
+          constructor... forwards* Hcomp: compatible_Ksubst __ K'.
           - forwards Htk1 : ok_term_ok_type Htype1. forwards Htk2 : ok_term_ok_type Htype2.
             forwards~ Hnin1 : ok_type_notin_K K' Htk1. forwards~ Hnin2 : ok_type_notin_K K' Htk2.
             simpls. rew_listx*. simpls~.
           - rew_listx* in Hcomp. }
-        { Case "TmSemApp". constructors*. apply* pats_exhaustive_Ksubst. }
+        { Case "TmSemApp". constructors*. apply* exhaustive_Ksubst. }
       Qed.
 
       Lemma ok_term_Kopen_change :
@@ -1666,6 +1807,9 @@ Module TypingProps (P : PAT).
         rewrite~ (Ksubst_t_intro K (FCon K')).
         rewrite~ <- (Ksubst_ty_fresh K (FCon K')).
         apply_empty~ ok_term_Ksubst.
+        forwards Henv : ok_term_ok_env Htype.
+        forwards (?&?&?&?&?&?) : ok_env_con_inv Henv. substs.
+        apply_fresh* EnvCon as K. applys* ok_env_concat.
       Qed.
 
     End TypingProps2.
